adjusting langs, universe libs

theories/lam/lang.v
@@ -1,17 +1,12 @@
 From iris.program_logic Require Export language ectx_language ectxi_language.
-From RunST Require Export base.
-From iris.prelude Require Import gmap.
+From st Require Export prelude.autosubst.
+From stdpp Require Export prelude.
 
-Local Open Scope Z_scope.
-
-(** Locations are defined as positive numbers *)
-Definition loc := positive.
-
-Instance loc_dec_eq (l l' : loc) : Decision (l = l') := _.
+(* Local Open Scope Z_scope. *)
 
 (** The litterals of the language *)
 Inductive base_lit : Set :=
-| LitInt (n : Z) | LitBool (b : bool) | LitUnit | LitLoc (l : loc).
+| LitInt (n : Z) | LitBool (b : bool) | LitUnit.
 
 Inductive bin_op : Set :=
 | PlusOp | MinusOp | LeOp | LtOp | EqOp.
@@ -19,6 +14,8 @@ Inductive bin_op : Set :=
 (** The syntax of expressions *)
 Inductive expr :=
 | Var (x : var)
+| LetIn (e : expr) (e : {bind 1 of expr})
+| Lam (e : {bind 1 of expr})
 | Rec (e : {bind 2 of expr})
 | App (e1 e2 : expr)
 (* Base Types *)
@@ -38,16 +35,26 @@ Inductive expr :=
 | Unfold (e : expr)
 (* Polymorphic Types *)
 | TLam (e : expr)
-| TApp (e : expr)
-(* Kleisli *)
-| Return (e: expr)
-| Bind (e1: expr) (e2: expr)
-| RunST (e: expr)
-(* Reference Types *)
-| Alloc (e : expr)
-| Read (e : expr)
-| Write (e1 : expr) (e2 : expr)
-| Compare (e1 : expr) (e2 : expr).
+| TApp (e : expr).
+
+Coercion LitInt : Z >-> base_lit.
+Coercion LitBool : bool >-> base_lit.
+Coercion Lit : base_lit >-> expr.
+Coercion App : expr >-> Funclass.
+Coercion Var : var >-> expr.
+
+Declare Scope expr_no_st_scope.
+Delimit Scope expr_no_st_scope with Eₙₒ.
+Notation "% x" := (Var x%nat) (at level 8, format "% x") : expr_no_st_scope.
+
+Notation "()" := (Lit LitUnit) : expr_no_st_scope.
+Notation "( e1 , e2 , .. , en )" := (Pair .. (Pair e1 e2) .. en) : expr_no_st_scope.
+
+Notation "e1 + e2" := (BinOp PlusOp e1%Eₙₒ e2%Eₙₒ) : expr_no_st_scope.
+Notation "e1 - e2" := (BinOp MinusOp e1%Eₙₒ e2%Eₙₒ) : expr_no_st_scope.
+Notation "e1 ≤ e2" := (BinOp LeOp e1%Eₙₒ e2%Eₙₒ) : expr_no_st_scope.
+Notation "e1 < e2" := (BinOp LtOp e1%Eₙₒ e2%Eₙₒ) : expr_no_st_scope.
+Notation "e1 = e2" := (BinOp EqOp e1%Eₙₒ e2%Eₙₒ) : expr_no_st_scope.
 
 Instance Ids_expr : Ids expr. derive. Defined.
 Instance Rename_expr : Rename expr. derive. Defined.
@@ -56,147 +63,60 @@ Instance SubstLemmas_expr : SubstLemmas expr. derive. Qed.
 
 (** Values for STLang *)
 Inductive val :=
+| LamV (e : {bind 1 of expr})
 | RecV (e : {bind 1 of expr})
 | TLamV (e : {bind 1 of expr})
-| ReturnV (v: val)
-| BindV (v1 v2: val)
 | LitV (v : base_lit)
 | PairV (v1 v2 : val)
 | InjLV (v : val)
 | InjRV (v : val)
-| FoldV (v : val)
-| AllocV (v : val)
-| ReadV (v : val)
-| WriteV (v1 v2 : val).
+| FoldV (v : val).
+
+Coercion LitV : base_lit >-> val.
+
+Declare Scope val_no_st_scope.
+Delimit Scope val_no_st_scope with Vₙₒ.
+
+Notation "()" := (LitV LitUnit) : val_no_st_scope.
+Notation "( v1 , v2 , .. , vn )" := (PairV .. (PairV v1 v2) .. vn) : val_no_st_scope.
 
 Fixpoint of_val (v : val) : expr :=
  match v with
+ | LamV e => Lam e
  | RecV e => Rec e
  | TLamV e => TLam e
- | ReturnV v => Return (of_val v)
- | BindV v1 v2 => Bind (of_val v1) (of_val v2)
  | LitV v => Lit v
  | PairV v1 v2 => Pair (of_val v1) (of_val v2)
  | InjLV v => InjL (of_val v)
  | InjRV v => InjR (of_val v)
  | FoldV v => Fold (of_val v)
- | AllocV v => Alloc (of_val v)
- | ReadV v => Read (of_val v)
- | WriteV v v' => Write (of_val v) (of_val v')
  end.
 
 Fixpoint to_val (e : expr) : option val :=
  match e with
+ | Lam e => Some (LamV e)
  | Rec e => Some (RecV e)
  | TLam e => Some (TLamV e)
- | Return e => v ← to_val e; Some (ReturnV v)
- | Bind e1 e2 => v1 ← to_val e1; v2 ← to_val e2; Some (BindV v1 v2)
  | Lit e => Some (LitV e)
  | Pair e1 e2 => v1 ← to_val e1; v2 ← to_val e2; Some (PairV v1 v2)
  | InjL e => InjLV <$> to_val e
  | InjR e => InjRV <$> to_val e
  | Fold e => v ← to_val e; Some (FoldV v)
- | Alloc e => v ← to_val e; Some (AllocV v)
- | Read e => v ← to_val e; Some (ReadV v)
- | Write e e' => v ← to_val e; v' ← to_val e'; Some (WriteV v v')
  | _ => None
  end.
 
-(** Contexts for the effectful language are of the form [Bind (Bind [] v2) v1] *)
-Inductive eff_ectx_item := BindECtx (v : val).
-
-(** A function that fills a context with an expression: *)
-Definition eff_fill_item (Ki : eff_ectx_item) (e : expr) : expr :=
- match Ki with BindECtx v => Bind e (of_val v) end.
-
-(** The state is defined as finite map from [loc] to [val]: *)
-Definition state := gmap loc val.
-
-(** Reduction relation for the effectful language *)
-Inductive eff_head_step :
-expr -> state -> expr -> state → list expr → Prop :=
-| ReadES l σ v :
-   σ !! l = Some v ->
-   eff_head_step (Read (Lit (LitLoc l))) σ (Return (of_val v)) σ []
-| WriteES σ l e v :
-   is_Some (σ !! l) -> to_val e = Some v ->
-   eff_head_step (Write (Lit (LitLoc l)) e)
-                  σ (Return (Lit LitUnit)) (<[l:=v]>σ) []
-| AllocES σ l e v :
-   (σ !! l) = None -> to_val e = Some v ->
-   eff_head_step (Alloc e) σ (Return (Lit (LitLoc l))) (<[l:=v]>σ) []
-| BindRetES σ v1 v2 e1 e2 :
-   to_val e1 = Some v1 -> to_val e2 = Some v2 ->
-   eff_head_step (Bind (Return e1) e2) σ (App e2 e1) σ [].
-
 Lemma to_of_val v : to_val (of_val v) = Some v.
 Proof.
- by induction v; simplify_option_eq; repeat f_equal; try apply (proof_irrel _).
+ by induction v; try simplify_option_eq; repeat f_equal; try apply (proof_irrel _).
 Qed.
 Lemma of_to_val e v : to_val e = Some v → of_val v = e.
 Proof.
  revert v; induction e; intros v ?; simplify_option_eq; auto with f_equal.
 Qed.
 
-(** Values for the effectful language: *)
-Inductive eff_val :=
-| ReturnEV (v : val)
-| AppCtxEV (K : list eff_ectx_item) (v1 v2 : val).
-
-Definition of_eff_val (ev : eff_val) : expr :=
-match ev with
-| ReturnEV w => Return (of_val w)
-| AppCtxEV K v1 v2 => fold_right eff_fill_item (App (of_val v1) (of_val v2)) K
-end.
-
-Instance maybe_AppCtxEV : Maybe3 AppCtxEV := λ ev,
- match ev with AppCtxEV K e1 e2 => Some (K, e1, e2) | _ => None end.
-
-Fixpoint to_eff_val (e : expr) : option eff_val :=
- match e with
- | Return e => v ← to_val e; Some (ReturnEV v)
- | App e e' => v ← to_val e; v' ← to_val e'; Some (AppCtxEV [] v v')
- | Bind e e' => '(K, v1, v2) ← to_eff_val e ≫= maybe3 AppCtxEV; v' ← to_val e';
-                 Some (AppCtxEV (BindECtx v' :: K) v1 v2)
- | _ => None
- end.
-
-Lemma to_of_eff_val v : to_eff_val (of_eff_val v) = Some v.
-Proof.
- destruct v as [|K v1 v2]; first by rewrite /= to_of_val.
- induction K as [|[]]; first rewrite /= !to_of_val //.
- rewrite /= IHK /= to_of_val //.
-Qed.
-
-Lemma of_to_eff_val e v : to_eff_val e = Some v → of_eff_val v = e.
-  revert v. induction e => v; rewrite //=.
-  - destruct (to_val e1) eqn:Heq1; rewrite //=;
-    destruct (to_val e2) eqn:Heq2; rewrite //=.
-    inversion 1; subst; simpl; erewrite !of_to_val; eauto.
- - destruct (to_val e) eqn:Heq1; rewrite //=.
-   inversion 1; subst; simpl; erewrite !of_to_val; eauto.
- - destruct (to_eff_val e1) as [[]|] eqn:Heq1; rewrite //=.
-   destruct (to_val e2) eqn:Heq2; rewrite //=. inversion 1; subst; simpl.
-   specialize (IHe1 (AppCtxEV K _ _) eq_refl). simpl in *. rewrite IHe1.
-   erewrite !of_to_val; eauto.
-Qed.
-
 (** Equality and other typeclass stuff *)
 Instance of_val_inj : Inj (=) (=) of_val.
 Proof. by intros ?? Hv; apply (inj Some); rewrite -!to_of_val Hv. Qed.
-Instance eff_of_val_inj : Inj (=) (=) of_eff_val.
-Proof.
- intros v; induction v => w.
- - destruct w; simpl.
-   + inversion 1; subst; f_equal; by apply of_val_inj.
-   + destruct K as [|[]]; done.
- - revert v1 v2 w. induction K as [|[] K'] => v1 v2 w; (destruct w; first done).
-   + destruct K as [|[] K]; inversion 1; f_equal; eauto using of_val_inj.
-   + destruct K as [|[]]; first done.
-     inversion 1 as [[Hb1 Hb2]].
-     specialize (IHK' _ _ (AppCtxEV K _ _) Hb1). inversion IHK'; subst.
-     erewrite of_val_inj; eauto.
-Qed.
 
 Instance base_lit_eq_dec : EqDecision base_lit.
 Proof. solve_decision. Defined.
@@ -209,77 +129,18 @@ Proof.
  refine (λ v v', cast_if (decide (of_val v = of_val v')));
    abstract naive_solver.
 Defined.
-Instance eff_val_eq_dec : EqDecision eff_val.
-Proof.
- refine (λ v v', cast_if (decide (of_eff_val v = of_eff_val v')));
-   abstract naive_solver.
-Defined.
 
 Instance expr_inhabited : Inhabited expr := populate (Lit LitUnit).
 Instance val_inhabited : Inhabited val := populate (LitV LitUnit).
-Canonical Structure stateC := leibnizC state.
-Canonical Structure valC := leibnizC val.
-Canonical Structure eff_valC := leibnizC eff_val.
-Canonical Structure exprC := leibnizC expr.
-
-Instance eff_fill_item_inj Ki : Inj (=) (=) (eff_fill_item Ki).
-Proof. destruct Ki; intros ???; simplify_eq/=; auto with f_equal. Qed.
-Lemma eff_fill_item_val Ki e :
- is_Some (to_eff_val (eff_fill_item Ki e)) → is_Some (to_eff_val e).
-Proof. intros [v ?]. destruct Ki; simplify_option_eq; eauto. Qed.
-Lemma eff_val_stuck e1 σ1 e2 σ2 efs :
- eff_head_step e1 σ1 e2 σ2 efs → to_eff_val e1 = None.
-Proof. destruct 1; try done. simpl; rewrite H H0; done. Qed.
-Lemma eff_head_ctx_step_val Ki e σ1 e2 σ2 efs :
- eff_head_step (eff_fill_item Ki e) σ1 e2 σ2 efs → is_Some (to_eff_val e).
-Proof. destruct Ki; inversion_clear 1; simplify_option_eq; by eauto. Qed.
-Lemma eff_fill_item_no_val_inj Ki1 Ki2 e1 e2 :
- to_eff_val e1 = None → to_eff_val e2 = None →
- eff_fill_item Ki1 e1 = eff_fill_item Ki2 e2 → Ki1 = Ki2.
-Proof.
- destruct Ki1, Ki2; intros; try discriminate; simplify_eq/=;
-  repeat match goal with
-  | H : to_val (of_val _) = None |- _ => by rewrite to_of_val in H
-  end; auto.
-Qed.
-
-(** Both languages share the same syntax: *)
-Definition eff_expr := expr.
-
-(** We declare that the effectful language is a language to Iris by giving the
- expressions, values, contexts and operations and lemmas on those. *)
-Program Instance eff_ectxi_lang :
- EctxiLanguage expr eff_val eff_ectx_item state := {|
-  ectxi_language.of_val := of_eff_val;
-  ectxi_language.to_val := to_eff_val;
-  ectxi_language.fill_item := eff_fill_item;
-  ectxi_language.head_step := eff_head_step
-|}.
-Solve Obligations with eauto using to_of_eff_val, of_to_eff_val,
- eff_val_stuck, eff_fill_item_val, eff_fill_item_no_val_inj,
- eff_head_ctx_step_val.
-
-Definition eff_ectx_lang := @EctxLanguage_instance_0 _ _ _ _ eff_ectxi_lang.
-
-Canonical Structure eff_lang := ectx_lang (eff_expr).
-
-Lemma eff_head_step_val σ (e : eff_expr) σ' e' efs :
-  language.prim_step e σ e' σ' efs → is_Some (to_val e).
-Proof.
- intros Hps. eapply prim_step_ind; eauto.
- intros K; revert e σ e' σ' Hps.
- induction K as [|[]]; intros e σ e' σ' Hps e1' e2' He He' Hps'.
- - inversion Hps' as []; subst; simpl; eauto;
-   repeat match goal with
-   | H : to_val _ = _ |- _ => rewrite H
-   end; simpl; eauto.
- - simpl; intros; subst. rewrite /= to_of_val /=.
-   edestruct (IHK (ectx_language.fill K e1')) as [? Heq]; eauto.
-   by apply Ectx_step'. simpl in *; rewrite Heq; eauto.
-Qed.
+(* Canonical Structure stateC := leibnizO state. *)
+(* Canonical Structure valC := leibnizO val. *)
+(* Canonical Structure eff_valC := leibnizO eff_val. *)
+(* Canonical Structure exprC := leibnizO expr. *)
 
 (** Evaluation contexts *)
 Inductive ectx_item :=
+| LetInLCtx (e2 : expr)
+| LetInRCtx (v1 : val)
 | AppLCtx (e2 : expr)
 | AppRCtx (v1 : val)
 | TAppCtx
@@ -294,20 +155,12 @@ Inductive ectx_item :=
 | BinOpLCtx (op : bin_op) (e2 : expr)
 | BinOpRCtx (op : bin_op) (v1 : val)
 | FoldCtx
-| UnfoldCtx
-| AllocCtx
-| ReadCtx
-| WriteLCtx (e2 : expr)
-| WriteRCtx (v1 : val)
-| ReturnCtx
-| BindLCtx (e2: expr)
-| BindRCtx (v1: val)
-| RunSTCtx
-| CompLCtx (e2 : expr)
-| CompRCtx (v1 : val).
+| UnfoldCtx.
 
 Definition fill_item (Ki : ectx_item) (e : expr) : expr :=
  match Ki with
+ | LetInLCtx e2 => LetIn e e2
+ | LetInRCtx v1 => LetIn (of_val v1) e
  | AppLCtx e2 => App e e2
  | AppRCtx v1 => App (of_val v1) e
  | TAppCtx => TApp e
@@ -323,93 +176,76 @@ Definition fill_item (Ki : ectx_item) (e : expr) : expr :=
  | BinOpRCtx op v1 => BinOp op (of_val v1) e
  | FoldCtx => Fold e
  | UnfoldCtx => Unfold e
- | AllocCtx => Alloc e
- | ReadCtx => Read e
- | WriteLCtx e2 => Write e e2
- | WriteRCtx v1 => Write (of_val v1) e
- | ReturnCtx => Return e
- | BindLCtx e2 => Bind e e2
- | BindRCtx v1 => Bind (of_val v1) e
- | RunSTCtx => RunST e
- | CompLCtx e2 => Compare e e2
- | CompRCtx v1 => Compare (of_val v1) e
  end.
 
 (** The stepping relation *)
 
 Definition bin_op_eval (op : bin_op) (z1 z2 : Z) : val :=
  match op with
- | PlusOp => LitV $ LitInt (z1 + z2)
+ | PlusOp => LitV $ LitInt (z1 + z2)%Z
  | MinusOp => LitV $ LitInt (z1 - z2)
- | LeOp => LitV $ LitBool $ bool_decide (z1 ≤ z2)
- | LtOp => LitV $ LitBool $ bool_decide (z1 < z2)
+ | LeOp => LitV $ LitBool $ bool_decide (z1 ≤ z2)%Z
+ | LtOp => LitV $ LitBool $ bool_decide (z1 < z2)%Z
  | EqOp => LitV $ LitBool $ bool_decide (z1 = z2)
  end.
 
-(** Reduction relation for STLang: *)
-Inductive head_step : expr → state → expr → state → list expr → Prop :=
-(* Embedding of the effectful language into STLang *)
-| EffS σ σ' (e : eff_expr) e':
-   language.prim_step e σ e' σ' [] ->
-   head_step (RunST e) σ (RunST e') σ' []
-| RunRet σ e v :
-    to_val e = Some v ->
-    head_step (RunST (Return e)) σ e σ []
-| Compare_suc σ l :
-    head_step
-      (Compare (Lit (LitLoc l)) (Lit (LitLoc l))) σ (Lit (LitBool true)) σ []
-| Compare_fail σ l l':
-    l ≠ l' →
-    head_step
-      (Compare (Lit (LitLoc l)) (Lit (LitLoc l'))) σ (Lit (LitBool false)) σ []
+Definition state : Type := ().
+
+Inductive head_step : expr → state → list Empty_set → expr → state → list expr → Prop :=
 (* β *)
-| BetaS e1 e2 v2 σ :
+  BetaLetIn e1 v1 e2 v2 σ κ :
+   to_val e1 = Some v1 →
    to_val e2 = Some v2 →
-   head_step (App (Rec e1) e2) σ e1.[(Rec e1), e2/] σ []
+   head_step (LetIn e1 e2) σ κ e2.[e1/] σ []
+| BetaLam e1 e2 v2 σ κ :
+   to_val e2 = Some v2 →
+   head_step (App (Lam e1) e2) σ κ e1.[e2/] σ []
+| BetaS e1 e2 v2 σ κ :
+   to_val e2 = Some v2 →
+   head_step (App (Rec e1) e2) σ κ e1.[(Rec e1), e2/] σ []
 (* binary operation *)
-| BinOpS op e1 e2 z1 z2 σ :
+| BinOpS op e1 e2 z1 z2 σ κ :
    to_val e1 = Some (LitV $ LitInt z1) → to_val e2 = Some (LitV $ LitInt z2) →
-   head_step (BinOp op e1 e2) σ (of_val (bin_op_eval op z1 z2)) σ []
+   head_step (BinOp op e1 e2) σ κ (of_val (bin_op_eval op z1 z2)) σ []
 (* if *)
-| IfTrueS e1 e2 σ :
-   head_step (If (Lit $ LitBool true) e1 e2) σ e1 σ []
-| IfFalseS e1 e2 σ :
-   head_step (If (Lit $ LitBool false) e1 e2) σ e2 σ []
+| IfTrueS e1 e2 σ κ :
+   head_step (If (Lit $ LitBool true) e1 e2) σ κ e1 σ []
+| IfFalseS e1 e2 σ κ :
+   head_step (If (Lit $ LitBool false) e1 e2) σ κ e2 σ []
 (* Products *)
-| FstS e1 v1 e2 v2 σ :
+| FstS e1 v1 e2 v2 σ κ :
    to_val e1 = Some v1 → to_val e2 = Some v2 →
-   head_step (Fst (Pair e1 e2)) σ e1 σ []
-| SndS e1 v1 e2 v2 σ :
+   head_step (Fst (Pair e1 e2)) σ κ e1 σ []
+| SndS e1 v1 e2 v2 σ κ :
    to_val e1 = Some v1 → to_val e2 = Some v2 →
-   head_step (Snd (Pair e1 e2)) σ e2 σ []
+   head_step (Snd (Pair e1 e2)) σ κ e2 σ []
 (* Sums *)
-| CaseLS e0 v0 e1 e2 σ :
+| CaseLS e0 v0 e1 e2 σ κ :
    to_val e0 = Some v0 →
-   head_step (Case (InjL e0) e1 e2) σ e1.[e0/] σ []
-| CaseRS e0 v0 e1 e2 σ :
+   head_step (Case (InjL e0) e1 e2) σ κ e1.[e0/] σ []
+| CaseRS e0 v0 e1 e2 σ κ :
    to_val e0 = Some v0 →
-   head_step (Case (InjR e0) e1 e2) σ e2.[e0/] σ []
+   head_step (Case (InjR e0) e1 e2) σ κ e2.[e0/] σ []
 (* Recursive Types *)
-| Unfold_Fold e v σ :
+| Unfold_Fold e v σ κ :
    to_val e = Some v →
-   head_step (Unfold (Fold e)) σ e σ []
+   head_step (Unfold (Fold e)) σ κ e σ []
 (* Polymorphic Types *)
-| TBeta e σ :
-   head_step (TApp (TLam e)) σ e σ [].
+| TBeta e σ κ :
+   head_step (TApp (TLam e)) σ κ e σ [].
 
 Instance fill_item_inj Ki : Inj (=) (=) (fill_item Ki).
 Proof. destruct Ki; intros ???; simplify_eq/=; auto with f_equal. Qed.
 Lemma fill_item_val Ki e :
  is_Some (to_val (fill_item Ki e)) → is_Some (to_val e).
 Proof. intros [v ?]. destruct Ki; simplify_option_eq; eauto. Qed.
-Lemma val_stuck e1 σ1 e2 σ2 efs :
- head_step e1 σ1 e2 σ2 efs → to_val e1 = None.
+Lemma val_stuck e1 σ1 κ e2 σ2 efs :
+ head_step e1 σ1 κ e2 σ2 efs → to_val e1 = None.
 Proof. destruct 1; done. Qed.
-Lemma head_ctx_step_val Ki e σ1 e2 σ2 efs :
- head_step (fill_item Ki e) σ1 e2 σ2 efs → is_Some (to_val e).
+Lemma head_ctx_step_val Ki e σ1 κ e2 σ2 efs :
+ head_step (fill_item Ki e) σ1 κ e2 σ2 efs → is_Some (to_val e).
 Proof.
- destruct Ki; inversion_clear 1; simplify_option_eq;
-  eauto using eff_head_step_val.
+ destruct Ki; inversion_clear 1; simplify_option_eq; eauto.
 Qed.
 Lemma fill_item_no_val_inj Ki1 Ki2 e1 e2 :
  to_val e1 = None → to_val e2 = None →
@@ -421,317 +257,25 @@ Proof.
   end; auto.
 Qed.
 
-(** Language *)
-Program Instance ST_ectxi_lang :
- EctxiLanguage expr val ectx_item state := {|
-  ectxi_language.of_val := of_val;
-  ectxi_language.to_val := to_val;
-  ectxi_language.fill_item := fill_item;
-  ectxi_language.head_step := head_step
-|}.
-Solve Obligations with eauto using to_of_val, of_to_val,
- val_stuck, fill_item_val, fill_item_no_val_inj,
- head_ctx_step_val.
-
-Definition ST_ectx_lang := @EctxLanguage_instance_0 _ _ _ _ ST_ectxi_lang.
-
-Canonical Structure ST_lang := ectx_lang (expr).
-
-Lemma ST_step_no_spawn e1 e2 σ1 σ2 nt:
-  @language.prim_step ST_lang e1 σ1 e2 σ2 nt -> nt = [].
+Lemma st_ectxi_lang_mixin : EctxiLanguageMixin of_val to_val fill_item head_step.
 Proof.
-  elim=> ? ? ? ? ? H. by elim: H.
+  split; eauto using to_of_val, of_to_val,
+  val_stuck, fill_item_val, fill_item_no_val_inj,
+ head_ctx_step_val, fill_item_inj.
 Qed.
 
-Lemma eff_step_no_spawn e1 e2 σ1 σ2 nt:
-  @language.prim_step eff_lang e1 σ1 e2 σ2 nt -> nt = [].
-Proof.
-  elim=> ? ? ? ? ? H. by elim: H.
-Qed.
+Canonical Structure lam_ectxi_lang : ectxiLanguage := EctxiLanguage st_ectxi_lang_mixin.
+Canonical Structure lam_ectx_lang : ectxLanguage := EctxLanguageOfEctxi lam_ectxi_lang.
+Canonical Structure lam_lang : language := LanguageOfEctx lam_ectx_lang.
 
-Lemma fill_val e K:
+Lemma fill_val (e : expr) (K : list ectx_item):
   is_Some (to_val (fill K e)) -> is_Some (to_val e).
 Proof.
   move=> [v h]. destruct (to_val e) eqn:eq.
     by exists v0.
-    have fill_not_val: to_val (fill K e) = None. by eauto using fill_not_val.
+    have fill_not_val: to_val (fill K e) = None. eauto using fill_not_val.
     congruence.
 Qed.
 
 Arguments val_stuck {_ _ _ _ _} _.
-Arguments eff_head_step_val {_ _ _ _ _} _.
-Arguments eff_step_no_spawn {_ _ _ _ _} _.
-Arguments ST_step_no_spawn {_ _ _ _ _} _.
 Arguments fill_val {_ _} _.
-
-
-Lemma step_runst_noval e σ1 e2 σ2 efs:
-  to_eff_val e = None ->
-  prim_step (RunST e) σ1 e2 σ2 efs ->
-  reducible (e: eff_expr) σ1 ->
-  ∃ e', e2 = RunST e' ∧ @language.prim_step eff_lang e σ1 e' σ2 efs.
-Proof.
-  intros enotval ps reduc. inversion ps; subst.
-  revert e1' H e2' H1 ps.
-  inversion reduc. destruct H as [σ' [efse Heffstep]].
-  have eval := eff_head_step_val Heffstep.
-  destruct K; simpl in *; subst; intros; subst.
-  - inversion H1; subst.
-    + exists e'. split; auto.
-    + simpl in *. rewrite H0 in enotval. discriminate.
-  - destruct e0; try discriminate. simpl in *. injection H; intro; subst.
-    have fill_val:= fill_val eval.
-    have hhh := val_stuck H1. rewrite hhh /is_Some in fill_val.
-    by destruct fill_val.
-Qed.
-
-Arguments step_runst_noval {_ _ _ _ _} _ _ _.
-
-Lemma alloc_fresh e v σ :
-	let l := fresh (dom _ σ) in
-	to_val e = Some v →
-        eff_head_step (Alloc e) σ (Return (Lit (LitLoc l))) (<[l:=v]>σ) [].
-Proof.
-  intros; apply: AllocES => //.
-    by apply (not_elem_of_dom (D:=gset _)), is_fresh.
-Qed.
-
-
-
-(** Deterministic version of the languages. We don't register these as
-instances/canonical structures to avoid confusion in resolutions. *)
-
-
-Inductive det_eff_head_step :
-  expr -> state -> expr -> state → list expr → Prop :=
-| det_ReadES l σ v :
-    σ !! l = Some v ->
-    det_eff_head_step (Read (Lit (LitLoc l))) σ (Return (of_val v)) σ []
-| det_WriteES σ l e v :
-    is_Some (σ !! l) -> to_val e = Some v ->
-    det_eff_head_step (Write (Lit (LitLoc l)) e)
-                  σ (Return (Lit LitUnit)) (<[l:=v]>σ) []
-| det_AllocES σ e v :
-    to_val e = Some v ->
-    det_eff_head_step
-      (Alloc e) σ
-      (Return (Lit (LitLoc (fresh (dom _ σ)))))
-      (<[(fresh (dom _ σ)):=v]>σ) []
-| det_BindRetES σ v1 v2 e1 e2 :
-    to_val e1 = Some v1 -> to_val e2 = Some v2 ->
-    det_eff_head_step (Bind (Return e1) e2) σ (App e2 e1) σ [].
-
-Lemma det_eff_head_step_eff_head_step e σ e' σ' es' :
-  det_eff_head_step e σ e' σ' es' → eff_head_step e σ e' σ' es'.
-Proof.
-  destruct 1; try econstructor; eauto.
-  eapply @not_elem_of_dom with (D := gset positive); first typeclasses eauto.
-  eapply is_fresh.
-Qed.
-
-Lemma det_eff_val_stuck e1 σ1 e2 σ2 efs :
- det_eff_head_step e1 σ1 e2 σ2 efs → to_eff_val e1 = None.
-Proof. destruct 1; try done. simpl; rewrite H H0; done. Qed.
-
-Lemma det_eff_head_ctx_step_val Ki e σ1 e2 σ2 efs :
- det_eff_head_step (eff_fill_item Ki e) σ1 e2 σ2 efs → is_Some (to_eff_val e).
-Proof. destruct Ki; inversion_clear 1; simplify_option_eq; by eauto. Qed.
-
-Lemma det_eff_head_step_det e σ e' σ' es' e'' σ'' es'' :
-  det_eff_head_step e σ e' σ' es' → det_eff_head_step e σ e'' σ'' es'' →
-  e' = e'' ∧ σ' = σ'' ∧ es' = es''.
-Proof.
-  intros H1; intros H2; destruct H1; inversion H2; subst;
-    match goal with
-      H1 : ?A = _, H2 : ?A = _ |- _ =>
-        by (rewrite H1 in H2; clear H1; inversion H2; subst)
-    end.
-Qed.
-
-Program Definition det_eff_ectxi_lang :
- EctxiLanguage expr eff_val eff_ectx_item state := {|
-  ectxi_language.of_val := of_eff_val;
-  ectxi_language.to_val := to_eff_val;
-  ectxi_language.fill_item := eff_fill_item;
-  ectxi_language.head_step := det_eff_head_step
-|}.
-Solve Obligations with eauto using to_of_eff_val, of_to_eff_val,
- det_eff_val_stuck, eff_fill_item_val, eff_fill_item_no_val_inj,
- det_eff_head_ctx_step_val.
-
-Definition det_eff_ectx_lang : EctxLanguage _ _ _ _ :=
-  (@EctxLanguage_instance_0 _ _ _ _ det_eff_ectxi_lang).
-
-Definition det_eff_lang : language := (@ectx_lang _ _ _ _ det_eff_ectx_lang).
-
-Lemma det_eff_head_step_val σ (e : eff_expr) σ' e' efs :
-  @language.prim_step det_eff_lang e σ e' σ' efs → is_Some (to_val e).
-Proof.
- intros Hps. eapply (@prim_step_ind _ _ _ _ det_eff_ectx_lang); eauto.
- intros K; revert e σ e' σ' Hps.
- induction K as [|[]]; intros e σ e' σ' Hps e1' e2' He He' Hps'.
- - inversion Hps' as []; subst; simpl; eauto;
-   repeat match goal with
-   | H : to_val _ = _ |- _ => rewrite H
-   end; simpl; eauto.
- - simpl; intros; subst. rewrite /= to_of_val /=.
-   edestruct (IHK (ectx_language.fill K e1')) as [? Heq]; eauto.
-   by apply (@Ectx_step' _ _ _ _ det_eff_ectx_lang).
-   simpl in *; rewrite Heq; eauto.
-Qed.
-
-Lemma eff_prim_step_impl e σ e' σ' es :
-  @language.prim_step det_eff_lang e σ e' σ' es →
-  @language.prim_step eff_lang e σ e' σ' es.
-Proof.
-  destruct 1; subst.
-  apply (@fill_step _ _ (@ectx_lang_ctx
-              _ _ _ _
-              (@EctxLanguage_instance_0 _ _ _ _ eff_ectxi_lang) K)).
-  apply head_prim_step.
-  simpl in *. by apply det_eff_head_step_eff_head_step.
-Qed.
-
-Lemma det_eff_prim_step_det e σ e' σ' es' e'' σ'' es'' :
-  @language.prim_step det_eff_lang e σ e' σ' es' →
-  @language.prim_step det_eff_lang e σ e'' σ'' es'' →
-  e' = e'' ∧ σ' = σ'' ∧ es' = es''.
-Proof.
-  intros H1 H2.
-  eapply (fun P => @prim_step_ind _ _ _ _ det_eff_ectx_lang _ _ _ _ _ _ P H1)
-  => K e1 e2 Heq1 Heq2 Hstp; subst.
-  apply fill_step_inv in H2; last eapply ectx_language.val_stuck; eauto.
-  destruct H2 as [e2' [-> H2]].
-  eapply (fun P => @prim_step_ind _ _ _ _ det_eff_ectx_lang _ _ _ _ _ _ P H2)
-  => K' e3 e4 Heq3 Heq4 Hstp'; subst.
-  assert (K' = []).
-  { destruct K' as [|k' K']; trivial; simpl in *.
-    apply det_eff_head_ctx_step_val in Hstp.
-    apply det_eff_val_stuck in Hstp'.
-    apply (@ectxi_language.fill_val _ _ _ _ det_eff_ectxi_lang K') in Hstp.
-    simpl in Hstp; rewrite Hstp' in Hstp; inversion Hstp; congruence. }
-  subst; simpl in *.
-  pose proof (det_eff_head_step_det _ _ _ _ _ _ _ _ Hstp Hstp'); firstorder.
-Qed.
-
-Lemma det_eff_no_prim_step_return e σ e' σ' es' :
-  is_Some (to_val e) →
-  @language.prim_step det_eff_lang (Return e) σ e' σ' es' → False.
-Proof.
-  intros Hnis Hps.
-  eapply (fun P => @prim_step_ind _ _ _ _ det_eff_ectx_lang _ _ _ _ _ _ P Hps)
-  => K e1 e2 Heq1 Heq2 Hstp; subst.
-  apply ectx_language.val_stuck in Hstp; simpl in *.
-  destruct K as [|[] K]; simpl in *; inversion Heq1; subst; simpl in *.
-  destruct (to_val e); inversion Hnis; simpl in *; try congruence.
-Qed.
-
-Inductive det_head_step : expr → state → expr → state → list expr → Prop :=
-| det_EffS σ σ' (e : eff_expr) e':
-    @language.prim_step det_eff_lang e σ e' σ' [] ->
-    det_head_step (RunST e) σ (RunST e') σ' []
-| det_RunRet σ e v :
-    to_val e = Some v ->
-   det_head_step (RunST (Return e)) σ e σ []
-| det_Compare_suc σ l :
-    det_head_step
-      (Compare (Lit (LitLoc l)) (Lit (LitLoc l))) σ (Lit (LitBool true)) σ []
-| det_Compare_fail σ l l':
-    l ≠ l' →
-    det_head_step
-      (Compare (Lit (LitLoc l)) (Lit (LitLoc l'))) σ (Lit (LitBool false)) σ []
-(* β *)
-| det_BetaS e1 e2 v2 σ :
-   to_val e2 = Some v2 →
-   det_head_step (App (Rec e1) e2) σ e1.[(Rec e1), e2/] σ []
-(* binary operation *)
-| det_BinOpS op e1 e2 z1 z2 σ :
-   to_val e1 = Some (LitV $ LitInt z1) → to_val e2 = Some (LitV $ LitInt z2) →
-   det_head_step (BinOp op e1 e2) σ (of_val (bin_op_eval op z1 z2)) σ []
-(* if *)
-| det_IfTrueS e1 e2 σ :
-   det_head_step (If (Lit $ LitBool true) e1 e2) σ e1 σ []
-| det_IfFalseS e1 e2 σ :
-   det_head_step (If (Lit $ LitBool false) e1 e2) σ e2 σ []
-(* Products *)
-| det_FstS e1 v1 e2 v2 σ :
-   to_val e1 = Some v1 → to_val e2 = Some v2 →
-   det_head_step (Fst (Pair e1 e2)) σ e1 σ []
-| det_SndS e1 v1 e2 v2 σ :
-   to_val e1 = Some v1 → to_val e2 = Some v2 →
-   det_head_step (Snd (Pair e1 e2)) σ e2 σ []
-(* Sums *)
-| det_CaseLS e0 v0 e1 e2 σ :
-   to_val e0 = Some v0 →
-   det_head_step (Case (InjL e0) e1 e2) σ e1.[e0/] σ []
-| det_CaseRS e0 v0 e1 e2 σ :
-   to_val e0 = Some v0 →
-   det_head_step (Case (InjR e0) e1 e2) σ e2.[e0/] σ []
-(* Recursive Types *)
-| det_Unfold_Fold e v σ :
-   to_val e = Some v →
-   det_head_step (Unfold (Fold e)) σ e σ []
-(* Polymorphic Types *)
-| det_TBeta e σ :
-    det_head_step (TApp (TLam e)) σ e σ [].
-
-Lemma det_head_step_head_step e σ e' σ' es' :
-  det_head_step e σ e' σ' es' → head_step e σ e' σ' es'.
-Proof.
-  destruct 1; try econstructor; eauto using eff_prim_step_impl.
-Qed.
-
-Lemma det_val_stuck e1 σ1 e2 σ2 efs :
- det_head_step e1 σ1 e2 σ2 efs → to_val e1 = None.
-Proof. destruct 1; done. Qed.
-Lemma det_head_ctx_step_val Ki e σ1 e2 σ2 efs :
- det_head_step (fill_item Ki e) σ1 e2 σ2 efs → is_Some (to_val e).
-Proof.
- destruct Ki; inversion_clear 1; simplify_option_eq;
-  eauto using det_eff_head_step_val.
-Qed.
-
-Lemma det_head_step_det e σ e' σ' es' e'' σ'' es'' :
-  det_head_step e σ e' σ' es' → det_head_step e σ e'' σ'' es'' →
-  e' = e'' ∧ σ' = σ'' ∧ es' = es''.
-Proof.
-  intros H1; intros H2; destruct H1;
-    inversion H2; subst; auto;
-      repeat match goal with
-               H1 : ?A = _, H2 : ?A = _ |- _ =>
-               rewrite H1 in H2; clear H1; inversion H2; subst
-             end; auto.
-  - pose proof (det_eff_prim_step_det _ _ _ _ _ _ _ _ H H1); firstorder.
-  - exfalso; eapply det_eff_no_prim_step_return; eauto.
-  - exfalso; eapply det_eff_no_prim_step_return; eauto.
-  - match goal with H : ?A ≠ ?A |- _ => by contradict H end.
-  - match goal with H : ?A ≠ ?A |- _ => by contradict H end.
-Qed.
-
-Program Definition det_ectxi_lang :
- EctxiLanguage expr val ectx_item state := {|
-  ectxi_language.of_val := of_val;
-  ectxi_language.to_val := to_val;
-  ectxi_language.fill_item := fill_item;
-  ectxi_language.head_step := det_head_step
-|}.
-Solve Obligations with eauto using to_of_val, of_to_val,
- det_val_stuck, fill_item_val, fill_item_no_val_inj,
- det_head_ctx_step_val.
-
-Definition det_ectx_lang : EctxLanguage _ _ _ _ :=
-  (@EctxLanguage_instance_0 _ _ _ _ det_ectxi_lang).
-
-Definition det_lang : language := (@ectx_lang _ _ _ _ det_ectx_lang).
-
-Lemma prim_step_impl e σ e' σ' es :
-  @language.prim_step det_lang e σ e' σ' es →
-  @language.prim_step ST_lang e σ e' σ' es.
-Proof.
-  destruct 1; subst.
-  apply (@fill_step _ _ (@ectx_lang_ctx
-              _ _ _ _
-              (@EctxLanguage_instance_0 _ _ _ _ ST_ectxi_lang) K)).
-  apply head_prim_step.
-  simpl in *. by apply det_head_step_head_step.
-Qed.
