theories/lam/typing.v
@@ -1,25 +1,4 @@
-From RunST Require Export lang.
-
-Inductive type :=
- | TUnit : type
- | TBool : type
- | TInt : type
- | TProd : type → type → type
- | TSum : type → type → type
- | TArrow : type → type → type
- | TRec (τ : {bind 1 of type})
- | TVar (x : var)
- | TForall (τ : {bind 1 of type})
- | TSTref (ρ τ : type)
- | TST (ρ τ : type).
-
-Global Instance type_eq_dec (τ τ' : type) : Decision (τ = τ').
-Proof. solve_decision. Defined.
-
-Instance Ids_type : Ids type. derive. Defined.
-Instance Rename_type : Rename type. derive. Defined.
-Instance Subst_type : Subst type. derive. Defined.
-Instance SubstLemmas_typer : SubstLemmas type. derive. Qed.
+From st.lam Require Export types lang.
 
 Definition binop_res_type (op : bin_op) : type :=
   match op with
@@ -27,60 +6,52 @@ Definition binop_res_type (op : bin_op) : type :=
   | EqOp => TBool | LeOp => TBool | LtOp => TBool
   end.
 
-Reserved Notation "Γ ⊢ₜ e : τ" (at level 74, e, τ at next level).
+Reserved Notation "Γ ⊢ₙₒ e : τ" (at level 74, e, τ at next level).
 
 Inductive typed (Γ : list type) : expr → type → Prop :=
- | TVar_typed x τ : Γ !! x = Some τ → Γ ⊢ₜ Var x : τ
- | TUnit_typed : Γ ⊢ₜ Lit (LitUnit) : TUnit
- | TBool_typed b : Γ ⊢ₜ Lit (LitBool b) : TBool
- | TInt_typed z : Γ ⊢ₜ Lit (LitInt z) : TInt
+ | Var_typed x τ : Γ !! x = Some τ → Γ ⊢ₙₒ Var x : τ
+ | Unit_typed : Γ ⊢ₙₒ Lit (LitUnit) : TUnit
+ | Bool_typed b : Γ ⊢ₙₒ Lit (LitBool b) : TBool
+ | Int_typed z : Γ ⊢ₙₒ Lit (LitInt z) : TInt
  | BinOp_typed op e1 e2 :
-     Γ ⊢ₜ e1 : TInt → Γ ⊢ₜ e2 : TInt → Γ ⊢ₜ BinOp op e1 e2 : binop_res_type op
+     Γ ⊢ₙₒ e1 : TInt → Γ ⊢ₙₒ e2 : TInt → Γ ⊢ₙₒ BinOp op e1 e2 : binop_res_type op
  | Pair_typed e1 e2 τ1 τ2 :
-    Γ ⊢ₜ e1 : τ1 → Γ ⊢ₜ e2 : τ2 → Γ ⊢ₜ Pair e1 e2 : TProd τ1 τ2
- | Fst_typed e τ1 τ2 : Γ ⊢ₜ e : TProd τ1 τ2 → Γ ⊢ₜ Fst e : τ1
- | Snd_typed e τ1 τ2 : Γ ⊢ₜ e : TProd τ1 τ2 → Γ ⊢ₜ Snd e : τ2
- | InjL_typed e τ1 τ2 : Γ ⊢ₜ e : τ1 → Γ ⊢ₜ InjL e : TSum τ1 τ2
- | InjR_typed e τ1 τ2 : Γ ⊢ₜ e : τ2 → Γ ⊢ₜ InjR e : TSum τ1 τ2
+    Γ ⊢ₙₒ e1 : τ1 → Γ ⊢ₙₒ e2 : τ2 → Γ ⊢ₙₒ Pair e1 e2 : TProd τ1 τ2
+ | Fst_typed e τ1 τ2 : Γ ⊢ₙₒ e : TProd τ1 τ2 → Γ ⊢ₙₒ Fst e : τ1
+ | Snd_typed e τ1 τ2 : Γ ⊢ₙₒ e : TProd τ1 τ2 → Γ ⊢ₙₒ Snd e : τ2
+ | InjL_typed e τ1 τ2 : Γ ⊢ₙₒ e : τ1 → Γ ⊢ₙₒ InjL e : τ1 + τ2
+ | InjR_typed e τ1 τ2 : Γ ⊢ₙₒ e : τ2 → Γ ⊢ₙₒ InjR e : TSum τ1 τ2
  | Case_typed e0 e1 e2 τ1 τ2 τ3 :
-    Γ ⊢ₜ e0 : TSum τ1 τ2 → τ1 :: Γ ⊢ₜ e1 : τ3 → τ2 :: Γ ⊢ₜ e2 : τ3 →
-    Γ ⊢ₜ Case e0 e1 e2 : τ3
+    Γ ⊢ₙₒ e0 : TSum τ1 τ2 → τ1 :: Γ ⊢ₙₒ e1 : τ3 → τ2 :: Γ ⊢ₙₒ e2 : τ3 →
+    Γ ⊢ₙₒ Case e0 e1 e2 : τ3
  | If_typed e0 e1 e2 τ :
-    Γ ⊢ₜ e0 : TBool → Γ ⊢ₜ e1 : τ → Γ ⊢ₜ e2 : τ → Γ ⊢ₜ If e0 e1 e2 : τ
+    Γ ⊢ₙₒ e0 : TBool → Γ ⊢ₙₒ e1 : τ → Γ ⊢ₙₒ e2 : τ → Γ ⊢ₙₒ If e0 e1 e2 : τ
+ | LetIn_typed e2 e1 τ1 τ2 :
+    τ1 :: Γ ⊢ₙₒ e2 : τ2 → Γ ⊢ₙₒ e1 : τ1 → Γ ⊢ₙₒ LetIn e1 e2 : τ2
+ | Lam_typed e τ1 τ2 :
+    τ1 :: Γ ⊢ₙₒ e : τ2 → Γ ⊢ₙₒ Lam e : TArrow τ1 τ2
  | Rec_typed e τ1 τ2 :
-    TArrow τ1 τ2 :: τ1 :: Γ ⊢ₜ e : τ2 → Γ ⊢ₜ Rec e : TArrow τ1 τ2
+    TArrow τ1 τ2 :: τ1 :: Γ ⊢ₙₒ e : τ2 → Γ ⊢ₙₒ Rec e : TArrow τ1 τ2
  | App_typed e1 e2 τ1 τ2 :
-    Γ ⊢ₜ e1 : TArrow τ1 τ2 → Γ ⊢ₜ e2 : τ1 → Γ ⊢ₜ App e1 e2 : τ2
+    Γ ⊢ₙₒ e1 : TArrow τ1 τ2 → Γ ⊢ₙₒ e2 : τ1 → Γ ⊢ₙₒ App e1 e2 : τ2
  | TLam_typed e τ :
-    subst (ren (+1)) <$> Γ ⊢ₜ e : τ → Γ ⊢ₜ TLam e : TForall τ
- | TApp_typed e τ τ' : Γ ⊢ₜ e : TForall τ → Γ ⊢ₜ TApp e : τ.[τ'/]
- | TFold e τ : Γ ⊢ₜ e : τ.[TRec τ/] → Γ ⊢ₜ Fold e : TRec τ
- | TUnfold e τ : Γ ⊢ₜ e : TRec τ → Γ ⊢ₜ Unfold e : τ.[TRec τ/]
- | TAlloc e τ ρ: Γ ⊢ₜ e : τ → Γ ⊢ₜ Alloc e : TST ρ (TSTref ρ τ)
- | TRead e τ ρ : Γ ⊢ₜ e : TSTref ρ τ → Γ ⊢ₜ Read e : TST ρ τ
- | TWrite e e' τ ρ :
-    Γ ⊢ₜ e : TSTref ρ τ → Γ ⊢ₜ e' : τ → Γ ⊢ₜ Write e e' : TST ρ TUnit
- | TBind e1 e2 ρ τ1 τ2 :
-    Γ ⊢ₜ e1 : TST ρ τ1 -> Γ ⊢ₜ e2 : (TArrow τ1 (TST ρ τ2)) ->
-    Γ ⊢ₜ (Bind e1 e2) : (TST ρ τ2)
- | TReturn e ρ τ : Γ ⊢ₜ e : τ -> Γ ⊢ₜ Return e : TST ρ τ
- | TRunST e τ :
-     subst (ren (+1)) <$>Γ ⊢ₜ e : TST (TVar 0) τ.[ren (+1)] ->
-     Γ ⊢ₜ RunST e : τ
- | TCompare e1 e2 ρ τ:
-     Γ ⊢ₜ e1 : TSTref ρ τ → Γ ⊢ₜ e2 : TSTref ρ τ → Γ ⊢ₜ Compare e1 e2 : TBool
-where "Γ ⊢ₜ e : τ" := (typed Γ e τ).
+    subst (ren (+1)) <$> Γ ⊢ₙₒ e : τ → Γ ⊢ₙₒ TLam e : TForall τ
+ | TApp_typed e τ τ' : Γ ⊢ₙₒ e : TForall τ → Γ ⊢ₙₒ TApp e : τ.[τ'/]
+ | Fold_typed e τ : Γ ⊢ₙₒ e : τ.[TRec τ/] → Γ ⊢ₙₒ Fold e : TRec τ
+ | Unfold_typed e τ : Γ ⊢ₙₒ e : TRec τ → Γ ⊢ₙₒ Unfold e : τ.[TRec τ/]
+where "Γ ⊢ₙₒ e : τ" := (typed Γ e τ%Tₙₒ).
 
 Lemma typed_subst_invariant Γ e τ s1 s2 :
-  Γ ⊢ₜ e : τ → (∀ x, x < length Γ → s1 x = s2 x) → e.[s1] = e.[s2].
+  Γ ⊢ₙₒ e : τ → (∀ x, x < length Γ → s1 x = s2 x) → e.[s1] = e.[s2].
 Proof.
   intros Htyped; revert s1 s2.
   assert (∀ x Γ, x < length (subst (ren (+1)) <$> Γ) → x < length Γ).
   { intros ??. by rewrite fmap_length. }
   assert (∀ {A} `{Ids A} `{Rename A} (s1 s2 : nat → A) x,
     (x ≠ 0 → s1 (pred x) = s2 (pred x)) → up s1 x = up s2 x).
-  { intros A H1 H2. rewrite /up=> s1 s2 [|x] //=; auto with f_equal omega. }
-  induction Htyped => s1 s2 Hs; f_equal/=; eauto using lookup_lt_Some with omega.
+  { intros A H1 H2. rewrite /up=> s1 s2 [|x] //=; auto with f_equal lia. }
+  induction Htyped => s1 s2 Hs; f_equal/=; eauto using lookup_lt_Some with lia;
+  apply IHHtyped; by rewrite fmap_length.
 Qed.
 Lemma n_closed_invariant n (e : expr) s1 s2 :
   (∀ f, e.[upn n f] = e) → (∀ x, x < n → s1 x = s2 x) → e.[s1] = e.[s2].
@@ -91,39 +62,89 @@ Proof.
     try (match goal with H : _ |- _ => eapply H end; eauto;
          try inversion Hmc; try match goal with H : _ |- _ => by rewrite H end;
          fail).
-  - apply H1. rewrite iter_up in Hmc. destruct lt_dec; try omega.
-    asimpl in *. cbv in x. replace (m + (x - m)) with x in Hmc by omega.
-    inversion Hmc; omega.
+  - apply H1. rewrite iter_up in Hmc. destruct lt_dec; try lia.
+    asimpl in *. cbv in x. replace (m + (x - m)) with x in Hmc by lia.
+    inversion Hmc; lia.
+  - apply (IHe0 (S m)).
+    + inversion Hmc. by do 2 rewrite H2.
+    + intro n. destruct n eqn:eq. by asimpl.
+      intro neq. asimpl. rewrite (H1 n0). by simpl. lia.
+  - unfold upn in *.
+    apply (IHe (S m)).
+    + inversion Hmc; match goal with H : _ |- _ => (by rewrite H) end.
+    + intros [|[|x]] H2; [by cbv| |].
+      asimpl; rewrite H1; auto with lia.
+      asimpl; rewrite H1; auto with lia.
   - unfold upn in *.
     change (e.[up (up (upn m (ren (+1))))]) with
     (e.[iter (S (S m)) up (ren (+1))]) in *.
     apply (IHe (S (S m))).
     + inversion Hmc; match goal with H : _ |- _ => (by rewrite H) end.
     + intros [|[|x]] H2; [by cbv|by cbv |].
-      asimpl; rewrite H1; auto with omega.
+      asimpl; rewrite H1; auto with lia.
   - change (e1.[up (upn m (ren (+1)))]) with
     (e1.[iter (S m) up (ren (+1))]) in *.
     apply (IHe0 (S m)).
     + inversion Hmc; match goal with H : _ |- _ => (by rewrite H) end.
     + intros [|x] H2; [by cbv |].
-      asimpl; rewrite H1; auto with omega.
+      asimpl; rewrite H1; auto with lia.
   - change (e2.[up (upn m (ren (+1)))]) with
     (e2.[upn (S m) (ren (+1))]) in *.
     apply (IHe1 (S m)).
     + inversion Hmc; match goal with H : _ |- _ => (by rewrite H) end.
     + intros [|x] H2; [by cbv |].
-      asimpl; rewrite H1; auto with omega.
+      asimpl; rewrite H1; auto with lia.
+Qed.
+
+Lemma n_closed_invariant_type n (e : type) s1 s2 :
+  (∀ f, e.[upn n f] = e) → (∀ x, x < n → s1 x = s2 x) → e.[s1] = e.[s2].
+Proof.
+  intros Hnc. specialize (Hnc (ren (+1))).
+  revert n Hnc s1 s2.
+  induction e => m Hmc s1 s2 H1; asimpl in *; try f_equal;
+    try (match goal with H : _ |- _ => eapply H end; eauto;
+         try inversion Hmc; try match goal with H : _ |- _ => by rewrite H end;
+         fail).
+  - unfold upn in *.
+    apply (IHe (S m)).
+    + inversion Hmc; match goal with H : _ |- _ => (by rewrite H) end.
+    + intros [|[|x]] H2; [by cbv| |].
+      asimpl; rewrite H1; auto with lia.
+      asimpl; rewrite H1; auto with lia.
+  - apply H1. rewrite iter_up in Hmc. destruct lt_dec; try lia.
+    asimpl in *. cbv in X. replace (m + (X - m)) with X in Hmc by lia.
+    inversion Hmc; lia.
+  - unfold upn in *.
+    apply (IHe (S m)).
+    + inversion Hmc; match goal with H : _ |- _ => (by rewrite H) end.
+    + intros [|[|x]] H2; [by cbv| |].
+      asimpl; rewrite H1; auto with lia.
+      asimpl; rewrite H1; auto with lia.
+Qed.
+
+Lemma subst_list_cons_closed_S_n_type (t : type) (ts : list type)
+        (tn : type) (Ctn : Closed_n (S (length ts)) tn) :
+  tn.[subst_list (t :: ts)] = tn.[up (subst_list ts)].[t/].
+Proof.
+  rewrite subst_comp. apply n_closed_invariant_type with (n := S (length ts)).
+  apply Ctn.
+  intros x px.
+  rewrite /subst_list.
+  destruct x. by asimpl.
+  asimpl. destruct (ts !! x) eqn:eq.
+  - simpl. by rewrite eq.
+  - assert (length ts ≤ x). by apply lookup_ge_None_1.
+    lia.
 Qed.
 
 Definition env_subst (vs : list val) (x : var) : expr :=
   from_option id (Var x) (of_val <$> vs !! x).
 
-Lemma typed_n_closed Γ τ e : Γ ⊢ₜ e : τ → (∀ f, e.[upn (length Γ) f] = e).
+Lemma typed_n_closed Γ τ e : Γ ⊢ₙₒ e : τ → (∀ f, e.[upn (length Γ) f] = e).
 Proof.
   intros H. induction H => f; asimpl; simpl in *; auto with f_equal.
-  - apply lookup_lt_Some in H. rewrite iter_up. destruct lt_dec; auto with omega.
+  - apply lookup_lt_Some in H. rewrite iter_up. destruct lt_dec; auto with lia.
   - f_equal. apply IHtyped.
-  - by f_equal; rewrite map_length in IHtyped.
   - by f_equal; rewrite map_length in IHtyped.
 Qed.
 
@@ -134,12 +155,12 @@ Lemma n_closed_subst_head_simpl n e w ws :
 Proof.
   intros H1 H2.
   rewrite /env_subst. eapply n_closed_invariant; eauto=> /= -[|x] ? //=.
-  destruct (lookup_lt_is_Some_2 ws x) as [v' Hv]; first omega; simpl.
+  destruct (lookup_lt_is_Some_2 ws x) as [v' Hv]; first lia; simpl.
   by rewrite Hv.
 Qed.
 
 Lemma typed_subst_head_simpl Δ τ e w ws :
-  Δ ⊢ₜ e : τ → length Δ = S (length ws) →
+  Δ ⊢ₙₒ e : τ → length Δ = S (length ws) →
   e.[of_val w .: env_subst ws] = e.[env_subst (w :: ws)].
 Proof. eauto using n_closed_subst_head_simpl, typed_n_closed. Qed.
 
@@ -149,12 +170,12 @@ Lemma n_closed_subst_head_simpl_2 n e w w' ws :
 Proof.
   intros H1 H2.
   rewrite /env_subst. eapply n_closed_invariant; eauto => /= -[|[|x]] H3 //=.
-  destruct (lookup_lt_is_Some_2 ws x) as [v' Hv]; first omega; simpl.
+  destruct (lookup_lt_is_Some_2 ws x) as [v' Hv]; first lia; simpl.
   by rewrite Hv.
 Qed.
 
 Lemma typed_subst_head_simpl_2 Δ τ e w w' ws :
-  Δ ⊢ₜ e : τ → length Δ = 2 + length ws →
+  Δ ⊢ₙₒ e : τ → length Δ = 2 + length ws →
   e.[of_val w .: of_val w' .: env_subst ws] = e.[env_subst (w :: w' :: ws)].
 Proof. eauto using n_closed_subst_head_simpl_2, typed_n_closed. Qed.
 
@@ -165,12 +186,12 @@ Lemma n_closed_subst_head_simpl_3 n e w1 w2 w3 ws :
 Proof.
   intros H1 H2.
   rewrite /env_subst. eapply n_closed_invariant; eauto => /= -[|[|[|x]]] H3 //=.
-  destruct (lookup_lt_is_Some_2 ws x) as [v' Hv]; first omega; simpl.
+  destruct (lookup_lt_is_Some_2 ws x) as [v' Hv]; first lia; simpl.
   by rewrite Hv.
 Qed.
 
 Lemma typed_subst_head_simpl_3 Δ τ e w1 w2 w3 ws :
-  Δ ⊢ₜ e : τ → length Δ = 3 + length ws →
+  Δ ⊢ₙₒ e : τ → length Δ = 3 + length ws →
   e.[of_val w1 .: of_val w2 .: of_val w3 .:env_subst ws] =
   e.[env_subst (w1 :: w2 :: w3 :: ws)].
 Proof. eauto using n_closed_subst_head_simpl_3, typed_n_closed. Qed.
@@ -182,12 +203,12 @@ Lemma n_closed_subst_head_simpl_4 n e w1 w2 w3 w4 ws :
 Proof.
   intros H1 H2.
   rewrite /env_subst. eapply n_closed_invariant; eauto => /= -[|[|[|[|x]]]] H3 //=.
-  destruct (lookup_lt_is_Some_2 ws x) as [v' Hv]; first omega; simpl.
+  destruct (lookup_lt_is_Some_2 ws x) as [v' Hv]; first lia; simpl.
   by rewrite Hv.
 Qed.
 
 Lemma typed_subst_head_simpl_4 Δ τ e w1 w2 w3 w4 ws :
-  Δ ⊢ₜ e : τ → length Δ = 4 + length ws →
+  Δ ⊢ₙₒ e : τ → length Δ = 4 + length ws →
   e.[of_val w1 .: of_val w2 .: of_val w3 .: of_val w4 .:env_subst ws] =
   e.[env_subst (w1 :: w2 :: w3 :: w4 :: ws)].
 Proof. eauto using n_closed_subst_head_simpl_4, typed_n_closed. Qed.
@@ -197,29 +218,25 @@ Proof. change (env_subst []) with (@ids expr _). by asimpl. Qed.
 
 (** Weakening *)
 Lemma context_gen_weakening ξ Γ' Γ e τ :
-  Γ' ++ Γ ⊢ₜ e : τ →
-  Γ' ++ ξ ++ Γ ⊢ₜ e.[upn (length Γ') (ren (+ (length ξ)))] : τ.
+  Γ' ++ Γ ⊢ₙₒ e : τ →
+  Γ' ++ ξ ++ Γ ⊢ₙₒ e.[upn (length Γ') (ren (+ (length ξ)))] : τ.
 Proof.
   intros H1.
   remember (Γ' ++ Γ) as Ξ. revert Γ' Γ ξ HeqΞ.
   induction H1 => Γ1 Γ2 ξ HeqΞ; subst; asimpl in *; eauto using typed.
   - rewrite iter_up; destruct lt_dec as [Hl | Hl].
     + constructor. rewrite lookup_app_l; trivial. by rewrite lookup_app_l in H.
-    + asimpl. constructor. rewrite lookup_app_r; auto with omega.
-      rewrite lookup_app_r; auto with omega.
-      rewrite lookup_app_r in H; auto with omega.
+    + asimpl. constructor. rewrite lookup_app_r; auto with lia.
+      rewrite lookup_app_r; auto with lia.
+      rewrite lookup_app_r in H; auto with lia.
       match goal with
-        |- _ !! ?A = _ => by replace A with (x - length Γ1) by omega
+        |- _ !! ?A = _ => by replace A with (x - length Γ1) by lia
       end.
   - econstructor; eauto. by apply (IHtyped2 (_::_)). by apply (IHtyped3 (_::_)).
+  - econstructor; eauto. by apply (IHtyped1 (_::_)).
+  - econstructor; eauto. by apply (IHtyped (_::_)).
   - constructor. by apply (IHtyped (_ :: _ :: _)).
   - constructor.
-    specialize (IHtyped
-      (subst (ren (+1)) <$> Γ1) (subst (ren (+1)) <$> Γ2) (subst (ren (+1)) <$> ξ)).
-    asimpl in *. rewrite ?map_length in IHtyped.
-    repeat rewrite fmap_app. apply IHtyped.
-    by repeat rewrite fmap_app.
-  - constructor; eauto.
     specialize (IHtyped
       (subst (ren (+1)) <$> Γ1) (subst (ren (+1)) <$> Γ2) (subst (ren (+1)) <$> ξ)).
     asimpl in *. rewrite ?map_length in IHtyped.
@@ -228,12 +245,12 @@ Proof.
 Qed.
 
 Lemma context_weakening ξ Γ e τ :
-  Γ ⊢ₜ e : τ → ξ ++ Γ ⊢ₜ e.[(ren (+ (length ξ)))] : τ.
+  Γ ⊢ₙₒ e : τ → ξ ++ Γ ⊢ₙₒ e.[(ren (+ (length ξ)))] : τ.
 Proof. eapply (context_gen_weakening _ []). Qed.
 
 Lemma context_gen_strengthening ξ Γ' Γ e τ :
-  Γ' ++ ξ ++ Γ ⊢ₜ e.[upn (length Γ') (ren (+ (length ξ)))] : τ →
-  Γ' ++ Γ ⊢ₜ e : τ.
+  Γ' ++ ξ ++ Γ ⊢ₙₒ e.[upn (length Γ') (ren (+ (length ξ)))] : τ →
+  Γ' ++ Γ ⊢ₙₒ e : τ.
 Proof.
   intros Ht.
   remember (Γ' ++ ξ ++ Γ) as Ξ.
@@ -249,19 +266,14 @@ Proof.
     + inversion Heqe'2; subst. rewrite lookup_app_l; auto.
       rewrite lookup_app_l in H; auto.
     + inversion Heqe'2; subst.
-      rewrite ?lookup_app_r in H; auto with omega.
-      rewrite lookup_app_r; auto with omega.
+      rewrite ?lookup_app_r in H; auto with lia.
+      rewrite lookup_app_r; auto with lia.
       replace (length Γ1 + length ξ + (x0 - length Γ1) - length Γ1 - length ξ)
-      with (x0 - length Γ1) in H; auto with omega.
+      with (x0 - length Γ1) in H; auto with lia.
   - econstructor; eauto. by eapply (IHHt2 (_::_)). by eapply (IHHt3 (_::_)).
+  - econstructor; eauto. by eapply (IHHt1 (_::_)).
+  - econstructor; eauto. by eapply (IHHt (_::_)).
   - econstructor; eauto. by eapply (IHHt (_ :: _::_)).
-  - constructor.
-    specialize (IHHt
-      (subst (ren (+1)) <$> Γ1) (subst (ren (+1)) <$> Γ2)
-      (subst (ren (+1)) <$> ξ)).
-    rewrite !map_length in IHHt.
-    repeat rewrite fmap_app. apply IHHt; auto.
-    by repeat rewrite fmap_app.
   - constructor.
     specialize (IHHt
       (subst (ren (+1)) <$> Γ1) (subst (ren (+1)) <$> Γ2)
@@ -272,7 +284,7 @@ Proof.
 Qed.
 
 Lemma context_strengthening ξ Γ e τ :
-  ξ ++ Γ ⊢ₜ e.[(ren (+ (length ξ)))] : τ → Γ ⊢ₜ e : τ.
+  ξ ++ Γ ⊢ₙₒ e.[(ren (+ (length ξ)))] : τ → Γ ⊢ₙₒ e : τ.
 Proof. eapply (context_gen_strengthening _ []). Qed.
 
 Definition swap_list n m : list nat := (seq n m) ++ seq 0 n.
@@ -288,7 +300,7 @@ Lemma lookup_n_swap_list_out n m i :
 Proof.
   rewrite /lookup_n /swap_list => Hge.
   rewrite lookup_ge_None_2; first done.
-  rewrite app_length !seq_length; omega.
+  rewrite app_length !seq_length; lia.
 Qed.
 
 Lemma lookup_n_swap_list_in n m i :
@@ -296,13 +308,13 @@ Lemma lookup_n_swap_list_in n m i :
 Proof.
   rewrite /lookup_n /swap_list => Hge.
   edestruct (@lookup_lt_is_Some_2 nat (seq n m ++ seq 0 n) i) as [x Hx].
-  { rewrite app_length !seq_length; omega. }
+  { rewrite app_length !seq_length; lia. }
   rewrite Hx.
   destruct (decide (i < m)).
   - rewrite lookup_app_l in Hx; last by rewrite seq_length.
-    apply lookup_seq_inv in Hx; omega.
-  - rewrite lookup_app_r in Hx; last rewrite seq_length; auto with omega.
-    apply lookup_seq_inv in Hx; omega.
+    apply lookup_seq in Hx; lia.
+  - rewrite lookup_app_r in Hx; last rewrite seq_length; auto with lia.
+    apply lookup_seq in Hx; lia.
 Qed.
 
 Lemma lookup_n_swap_list_r n m i :
@@ -310,20 +322,20 @@ Lemma lookup_n_swap_list_r n m i :
 Proof.
   rewrite /lookup_n /swap_list => Hlt.
   rewrite lookup_app_l; last by rewrite seq_length.
-  rewrite lookup_seq; auto.
+  rewrite lookup_seq_lt; auto.
 Qed.
 
 Lemma lookup_n_swap_list_l n m i :
   m ≤ i → i < n + m → lookup_n (swap_list n m) i = (i - m).
 Proof.
   rewrite /lookup_n /swap_list => Hle Hlt.
-  rewrite lookup_app_r; last rewrite seq_length; try omega.
-  rewrite lookup_seq; rewrite ?seq_length; auto with omega.
+  rewrite lookup_app_r; last rewrite seq_length; try lia.
+  rewrite lookup_seq_lt; rewrite ?seq_length; auto with lia.
 Qed.
 
 Lemma context_swap_typed Γ' ξ' ξ Γ e τ :
-  Γ' ++ ξ' ++ ξ ++ Γ ⊢ₜ e : τ →
-  Γ' ++ ξ ++ ξ' ++ Γ ⊢ₜ e.[upn (length Γ') (ren (lookup_n (swap_list (length ξ) (length ξ'))))] : τ.
+  Γ' ++ ξ' ++ ξ ++ Γ ⊢ₙₒ e : τ →
+  Γ' ++ ξ ++ ξ' ++ Γ ⊢ₙₒ e.[upn (length Γ') (ren (lookup_n (swap_list (length ξ) (length ξ'))))] : τ.
 Proof.
   intros Ht.
   remember (Γ' ++ ξ' ++ ξ ++ Γ) as Ξ. revert Γ' ξ' ξ Γ HeqΞ.
@@ -334,43 +346,41 @@ Proof.
         H : _ !! _ = Some _ |- _ => revert H
       end.
       rewrite !lookup_app_l; auto.
-    + constructor. simpl. rewrite lookup_app_r; auto with omega.
+    + constructor. simpl. rewrite lookup_app_r; auto with lia.
       replace (length Γ' + lookup_n (swap_list (length ξ) (length ξ')) (x - length Γ') - length Γ') with
-      (lookup_n (swap_list (length ξ) (length ξ')) (x - length Γ')) by omega.
+      (lookup_n (swap_list (length ξ) (length ξ')) (x - length Γ')) by lia.
       match goal with
         H : _ !! _ = Some _ |- _ =>
-        rewrite lookup_app_r in H; auto with omega; rename H into Hlu
+        rewrite lookup_app_r in H; auto with lia; rename H into Hlu
       end.
       destruct (decide ((x - length Γ') < (length ξ) + (length ξ'))).
       * rewrite app_assoc. rewrite app_assoc in Hlu.
         rewrite lookup_app_l; rewrite lookup_app_l in Hlu;
-          rewrite ?app_length; eauto with omega; try apply lookup_n_swap_list_in; auto.
+          rewrite ?app_length; eauto with lia; try apply lookup_n_swap_list_in; auto.
         destruct (decide ((x - length Γ') < (length ξ'))).
         -- rewrite lookup_n_swap_list_r; auto.
-           rewrite lookup_app_r; rewrite lookup_app_l in Hlu; auto with omega.
-           replace (length ξ + (x - length Γ') - length ξ) with (x - length Γ') by omega.
+           rewrite lookup_app_r; rewrite lookup_app_l in Hlu; auto with lia.
+           replace (length ξ + (x - length Γ') - length ξ) with (x - length Γ') by lia.
            done.
-        -- rewrite lookup_n_swap_list_l; auto with omega.
-           rewrite lookup_app_l; rewrite lookup_app_r in Hlu; auto with omega.
-      * rewrite lookup_n_swap_list_out; auto with omega.
+        -- rewrite lookup_n_swap_list_l; auto with lia.
+           rewrite lookup_app_l; rewrite lookup_app_r in Hlu; auto with lia.
+      * rewrite lookup_n_swap_list_out; auto with lia.
         rewrite app_assoc. rewrite app_assoc in Hlu.
         rewrite lookup_app_r; rewrite lookup_app_r in Hlu;
-          rewrite ?app_length; try rewrite ?app_length in Hlu; auto with omega.
+          rewrite ?app_length; try rewrite ?app_length in Hlu; auto with lia.
         replace (x - length Γ' - (length ξ + length ξ')) with
-        (x - length Γ' - (length ξ' + length ξ)) by omega.
+        (x - length Γ' - (length ξ' + length ξ)) by lia.
         done.
   - econstructor; eauto.
     + eapply (IHHt2 (_ :: _)). by simpl; f_equal.
     + eapply (IHHt3 (_ :: _)). by simpl; f_equal.
+  - econstructor.
+    + apply (IHHt1 (_ :: _)). by simpl; repeat f_equal.
+    + apply (IHHt2). by simpl; repeat f_equal.
+  - econstructor.
+    + apply (IHHt (_ :: _)). by simpl; repeat f_equal.
   - econstructor. apply (IHHt (_ :: _ :: _)). by simpl; repeat f_equal.
   - constructor.
-    specialize (IHHt
-      (subst (ren (+1)) <$> Γ') (subst (ren (+1)) <$> ξ')
-      (subst (ren (+1)) <$> ξ) (subst (ren (+1)) <$> Γ1)).
-    asimpl in *. rewrite ?map_length in IHHt.
-    repeat rewrite fmap_app. eapply IHHt.
-    by rewrite HeqΞ; repeat rewrite fmap_app.
-  - econstructor; eauto.
     specialize (IHHt
       (subst (ren (+1)) <$> Γ') (subst (ren (+1)) <$> ξ')
       (subst (ren (+1)) <$> ξ) (subst (ren (+1)) <$> Γ1)).
@@ -380,7 +390,7 @@ Proof.
 Qed.
 
 Lemma closed_context_weakening ξ Γ e τ :
-  (∀ f, e.[f] = e) → Γ ⊢ₜ e : τ → ξ ++ Γ ⊢ₜ e : τ.
+  (∀ f, e.[f] = e) → Γ ⊢ₙₒ e : τ → ξ ++ Γ ⊢ₙₒ e : τ.
 Proof. intros H1 H2. erewrite <- H1. by eapply context_weakening. Qed.
 
 Require Import Coq.Logic.FunctionalExtensionality.
@@ -394,7 +404,7 @@ Proof.
 Qed.
 
 Lemma context_gen_rename Γ e τ n m :
-  Γ ⊢ₜ e : τ → subst (upn n (ren (+m))) <$> Γ ⊢ₜ
+  Γ ⊢ₙₒ e : τ → subst (upn n (ren (+m))) <$> Γ ⊢ₙₒ
                      e : τ.[upn n (ren (+m))].
 Proof.
   intros Ht. revert n m.
@@ -419,23 +429,18 @@ Proof.
     replace (τ.[TRec τ/].[upn n (ren (+m))]) with
     (τ.[upn (S n) (ren (+m))].[TRec τ.[upn (S n) (ren (+m))]/]) by by asimpl.
     by econstructor.
-  - specialize (IHHt (S n) m). asimpl in IHHt.
-    econstructor. asimpl.
-    rewrite -list_fmap_compose /compose in IHHt.
-    rewrite -list_fmap_compose /compose.
-    by rewrite -ren_upn_ren.
 Qed.
 
 Lemma context_rename Γ e τ m :
-  Γ ⊢ₜ e : τ → subst (ren (+m)) <$> Γ ⊢ₜ e : τ.[ren (+m)].
+  Γ ⊢ₙₒ e : τ → subst (ren (+m)) <$> Γ ⊢ₙₒ e : τ.[ren (+m)].
 Proof.
   eapply (context_gen_rename _ _ _ 0).
 Qed.
 
 Lemma typed_gen_subst Γ1 Γ2 e1 τ1 e2 τ2 :
-  Γ1 ++ τ2 :: Γ2 ⊢ₜ e1 : τ1 →
-  Γ2 ⊢ₜ e2 : τ2 →
-  Γ1 ++ Γ2 ⊢ₜ e1.[upn (length Γ1) (e2 .: ids)] : τ1.
+  Γ1 ++ τ2 :: Γ2 ⊢ₙₒ e1 : τ1 →
+  Γ2 ⊢ₙₒ e2 : τ2 →
+  Γ1 ++ Γ2 ⊢ₙₒ e1.[upn (length Γ1) (e2 .: ids)] : τ1.
 Proof.
   remember (Γ1 ++ τ2 :: Γ2) as ξ. intros Ht. revert Γ1 Γ2 e2 τ2 Heqξ.
   induction Ht => Γ1 Γ2 oe2 oτ2 Heqξ; asimpl in *; eauto using typed.
@@ -448,14 +453,14 @@ Proof.
     + asimpl. remember (x - length Γ1) as n. destruct n.
        * match goal with
            H : (Γ1 ++ oτ2 :: Γ2) !! x = Some τ |- _ =>
-           rewrite lookup_app_r in H; auto with omega; rewrite -Heqn in H;
+           rewrite lookup_app_r in H; auto with lia; rewrite -Heqn in H;
              inversion H; subst
          end.
          by apply context_weakening.
        * asimpl.
          match goal with
            H : (Γ1 ++ oτ2 :: Γ2) !! x = Some τ |- _ =>
-           rewrite lookup_app_r in H; auto with omega; rewrite -Heqn in H;
+           rewrite lookup_app_r in H; auto with lia; rewrite -Heqn in H;
              inversion H; subst
          end.
          change (ids (length Γ1 + n)) with (@ids expr _ n).[ren (+(length Γ1))].
@@ -463,14 +468,12 @@ Proof.
   - econstructor; eauto.
     + eapply (IHHt2 (_ :: _)); eauto; by simpl; f_equal.
     + eapply (IHHt3 (_ :: _)); eauto; by simpl; f_equal.
+  - econstructor; eauto.
+    eapply (IHHt1 (_ :: _)); eauto; by simpl; f_equal.
+  - econstructor; eauto.
+    eapply (IHHt (_ :: _)); eauto; by simpl; f_equal.
   - econstructor. eapply (IHHt (_ :: _ :: _)); eauto; by simpl; repeat f_equal.
   - constructor.
-    specialize (IHHt
-      (subst (ren (+1)) <$> Γ1) (subst (ren (+1)) <$> Γ2)).
-    asimpl in *. rewrite ?map_length in IHHt.
-    repeat rewrite fmap_app. eapply IHHt; eauto using context_rename.
-    by rewrite Heqξ; repeat rewrite fmap_app.
-  - econstructor; eauto.
     specialize (IHHt
       (subst (ren (+1)) <$> Γ1) (subst (ren (+1)) <$> Γ2)).
     asimpl in *. rewrite ?map_length in IHHt.
@@ -479,5 +482,5 @@ Proof.
 Qed.
 
 Lemma typed_subst Γ2 e1 τ1 e2 τ2 :
-  τ2 :: Γ2 ⊢ₜ e1 : τ1 → Γ2 ⊢ₜ e2 : τ2 → Γ2 ⊢ₜ e1.[e2/] : τ1.
+  τ2 :: Γ2 ⊢ₙₒ e1 : τ1 → Γ2 ⊢ₙₒ e2 : τ2 → Γ2 ⊢ₙₒ e1.[e2/] : τ1.
 Proof. apply (typed_gen_subst []). Qed.
