theories/prelude/autosubst.v
@@ -1,6 +1,5 @@
-Require Export Utf8_core.
-From iris Require Export base.
-
+From stdpp Require Export prelude.
+From iris Require Export prelude.
 From Autosubst Require Export Autosubst.
 
 Section Autosubst_Lemmas.
@@ -34,5 +33,41 @@ Section Autosubst_Lemmas.
       + by asimpl.
       + asimpl. rewrite IHn. by asimpl. lia.
   Qed.
+
+  Definition Closed_n (n : nat) (t : term) : Prop := ∀ σ, t.[upn n σ] = t.
+  Definition Closed : term → Prop := Closed_n 0.
+
+  Definition subst_list (vs : list term) : var → term :=
+    fun (x : var) => from_option id (ids x) (vs !! x).
+
+  Lemma simul_subst_closed (s t1 t2 : term) (Ct1 : Closed t1) (Ct2 : Closed t2) : s.[t1/].[t2/] = s.[t1,t2/].
+  Proof. asimpl. by rewrite Ct1. Qed.
+
+  Lemma scomp_closed_term (t : term) (Ct : Closed t) σ : t .: σ = t .: ids >> σ.
+  Proof.
+    f_ext. intro x. induction x.
+    - by simpl.
+    - by asimpl.
+  Qed.
+
+  (* Lemma n_closed_invariant n (e : term) s1 s2 : *)
+  (*   Closed_n n e → (∀ x, x < n → s1 x = s2 x) → e.[s1] = e.[s2]. *)
+  (* Proof. *)
+  (* Admitted. *)
+
+  (* Lemma subst_list_cons_closed_S_n (t : term) (ts : list term) *)
+  (*        (tn : term) (Ctn : Closed_n (S (length ts)) tn) : *)
+  (*   tn.[subst_list (t :: ts)] = tn.[up (subst_list ts)].[t/]. *)
+  (* Proof. *)
+  (*   rewrite subst_comp. apply n_closed_invariant with (n := S (length ts)). *)
+  (*   apply Ctn. *)
+  (*   intros x px. *)
+  (*   rewrite /subst_list. *)
+  (*   destruct x. by asimpl. *)
+  (*   asimpl. destruct (ts !! x) eqn:eq. *)
+  (*   - simpl. by rewrite eq. *)
+  (*   - assert (length ts ≤ x). by apply lookup_ge_None_1. *)
+  (*     lia. *)
+  (* Qed. *)
 
 End Autosubst_Lemmas.
