theories/lam/lib/dummy.v
@@ -1,0 +1,4 @@
+From st.lam Require Export lang.
+
+Definition dummy : expr.
+Proof. exact ()%Eₙₒ. Qed.
