theories/lam/lib/omega.v
@@ -1,0 +1,13 @@
+From st.lam Require Export types lang typing.
+
+Definition Ω : expr :=
+  (Rec (%0 %1) ())%Eₙₒ.
+
+Lemma Ω_loop σ κ : prim_step Ω σ κ Ω σ [].
+Proof. apply head_prim_step. rewrite /Ω. by eapply BetaS. Qed.
+
+Lemma Ω_typed Γ τ : Γ ⊢ₙₒ Ω : τ.
+Proof.
+  rewrite /Ω. eapply App_typed; try by constructor.
+  apply Rec_typed. eapply App_typed; by constructor.
+Qed.
