theories/lam/lib/universe.v
@@ -1,0 +1,232 @@
+From st.lam Require Export types lang typing.
+From st.lam.lib Require Export omega fixlam dummy.
+
+(* Local Open Scope Eₙₒ. *)
+(* Local Open Scope Tₙₒ. *)
+
+Definition TUniverse_body : type :=
+  (( TUnit +
+   TBool +
+   TInt +
+   (TVar 0 × TVar 0) +
+   (TVar 0 + TVar 0) +
+   (TVar 0 ⟶ TVar 0) ) +
+   TRec (TVar 1)
+  )%Tₙₒ.
+
+Definition TUniverse : type := TRec TUniverse_body.
+
+Definition TUniverse_unfolded : type := TUniverse_body.[TUniverse/].
+
+From st Require Export lang.
+
+Inductive type_constructor :=
+  | TCUnit
+  | TCBool
+  | TCInt
+  | TCProd
+  | TCSum
+  | TCArrow
+  | TCRec.
+
+Definition type_constructor_branch (tc : type_constructor) : type :=
+  match tc with
+  | TCUnit => TUnit
+  | TCBool => TBool
+  | TCInt => TInt
+  | TCSum => (TUniverse + TUniverse)%Tₙₒ
+  | TCProd => (TUniverse × TUniverse)%Tₙₒ
+  | TCArrow => (TUniverse ⟶ TUniverse)%Tₙₒ
+  | TCRec => TRec TUniverse
+  end.
+
+Definition InjTC (tc : type_constructor) (e : expr) : expr :=
+  match tc with
+  | TCUnit => InjL (InjL (InjL (InjL (InjL (InjL e)))))
+  | TCBool => InjL (InjL (InjL (InjL (InjL (InjR e)))))
+  | TCInt => InjL (InjL (InjL (InjL (InjR e))))
+  | TCProd => InjL (InjL (InjL (InjR e)))
+  | TCSum => InjL (InjL (InjR e))
+  | TCArrow => InjL (InjR e)
+  | TCRec => InjR e
+  end.
+
+Definition InjVTC (tc : type_constructor) (v : val) : val :=
+  match tc with
+  | TCUnit => InjLV (InjLV (InjLV (InjLV (InjLV (InjLV v)))))
+  | TCBool => InjLV (InjLV (InjLV (InjLV (InjLV (InjRV v)))))
+  | TCInt => InjLV (InjLV (InjLV (InjLV (InjRV v))))
+  | TCProd => InjLV (InjLV (InjLV (InjRV v)))
+  | TCSum => InjLV (InjLV (InjRV v))
+  | TCArrow => InjLV (InjRV v)
+  | TCRec => InjRV v
+  end.
+
+Lemma InjTC_typed (tc : type_constructor) (e : expr) Γ (d : Γ ⊢ₙₒ e : type_constructor_branch tc) :
+  Γ ⊢ₙₒ InjTC tc e : TUniverse_unfolded.
+Proof. destruct tc; by repeat constructor. Proof. Qed.
+
+Definition CaseTC (tc : type_constructor) (e : expr) : expr :=
+  match tc with
+  | TCUnit => Case e (Case %0 (Case %0 (Case %0 (Case %0 (Case %0 %0 Ω) Ω) Ω) Ω) Ω)%Eₙₒ Ω
+  | TCBool => Case e (Case %0 (Case %0 (Case %0 (Case %0 (Case %0 Ω %0) Ω) Ω) Ω) Ω)%Eₙₒ Ω
+  | TCInt => Case e (Case %0 (Case %0 (Case %0 (Case %0 Ω %0) Ω) Ω) Ω)%Eₙₒ Ω
+  | TCProd => Case e (Case %0 (Case %0 (Case %0 Ω %0) Ω) Ω)%Eₙₒ Ω
+  | TCSum => Case e (Case %0 (Case %0 Ω %0) Ω)%Eₙₒ Ω
+  | TCArrow => Case e (Case %0 Ω %0)%Eₙₒ Ω
+  | TCRec => (Case e Ω %0)%Eₙₒ
+  end.
+
+Lemma CaseTC_typed (tc : type_constructor) (e : expr) Γ (d : Γ ⊢ₙₒ e : TUniverse_unfolded) :
+  Γ ⊢ₙₒ CaseTC tc e : type_constructor_branch tc.
+Proof. destruct tc; repeat eapply Case_typed; (by constructor) || (by apply Ω_typed) || (try by eapply d). Qed.
+
+(* Definition inject (tc : type_constructor) (e : expr) : expr := Fold (InjTC tc e). *)
+
+(* Lemma inject_typed (tc : type_constructor) (e : expr) Γ (d : Γ ⊢ₙₒ e : type_constructor_branch tc) : *)
+(*   Γ ⊢ₙₒ inject tc e : TUniverse. *)
+(* Proof. by apply Fold_typed, InjTC_typed. Qed. *)
+
+(* Definition extract (tc : type_constructor) (e : expr) : expr := (CaseTC tc (Unfold e)). *)
+
+(* Lemma extract_typed (tc : type_constructor) (e : expr) Γ (d : Γ ⊢ₙₒ e : TUniverse) : *)
+(*   Γ ⊢ₙₒ extract tc e : type_constructor_branch tc. *)
+(* Proof. by apply CaseTC_typed, Unfold_typed. Qed. *)
+
+Definition inject (tc : type_constructor) : expr := Lam (Fold (InjTC tc %0))%Eₙₒ.
+
+Lemma inject_typed (tc : type_constructor) Γ :
+  Γ ⊢ₙₒ inject tc : type_constructor_branch tc ⟶ TUniverse.
+Proof. by apply Lam_typed, Fold_typed, InjTC_typed, Var_typed. Qed.
+
+Definition extract (tc : type_constructor) : expr := Lam (CaseTC tc (Unfold %0))%Eₙₒ.
+
+Lemma extract_typed (tc : type_constructor) Γ :
+  Γ ⊢ₙₒ extract tc : TUniverse ⟶ type_constructor_branch tc.
+Proof. by apply Lam_typed, CaseTC_typed, Unfold_typed, Var_typed. Qed.
+
+Inductive direction :=
+  | upward
+  | downward.
+
+Fixpoint embed_project_pair (xs : list var) (τ : type) : expr :=
+  match τ with
+  | TUnit => (inject TCUnit , extract TCUnit)%Eₙₒ
+  | TBool => (inject TCBool , extract TCBool)%Eₙₒ
+  | TInt => (inject TCInt , extract TCInt)%Eₙₒ
+  | TProd τ1 τ2 => (Lam (LetIn (Fst %0) (LetIn (Snd %1)
+                                              (inject TCProd (Fst (embed_project_pair ((+3) <$> xs) τ1) %1, Fst (embed_project_pair ((+3) <$> xs) τ2) %0)))) ,
+                   Lam (LetIn (extract TCProd %0) (LetIn (Fst %0) (LetIn (Snd %1)
+                                                                         (Snd (embed_project_pair ((+4) <$> xs) τ1) %1 , Snd (embed_project_pair ((+4) <$> xs) τ2) %0)))))%Eₙₒ
+  | TSum τ1 τ2 => (Lam (Case %0 (inject TCSum (InjL (Fst (embed_project_pair ((+2) <$> xs) τ1) %0))) (inject TCSum (InjR (Fst (embed_project_pair ((+2) <$> xs) τ2) %0)))) ,
+                  (Lam (Case (extract TCSum %0) (InjL (Snd (embed_project_pair ((+2) <$> xs) τ1) %0)) (InjR (Snd (embed_project_pair ((+2) <$> xs) τ2) %0)))))%Eₙₒ
+  | TArrow τ1 τ2 => (Lam (inject TCArrow (Lam (Fst (embed_project_pair ((+2) <$> xs) τ2) (%1 (Snd (embed_project_pair ((+2) <$> xs) τ1) %0))))) ,
+                    (Lam (Lam (Snd (embed_project_pair ((+2) <$> xs) τ2) (extract TCArrow %1 (Fst (embed_project_pair ((+2) <$> xs) τ1) %0))))))%Eₙₒ
+  | TRec τ => FixLam (Lam (inject TCRec (Fold (Fst (embed_project_pair (1 :: ((+2) <$> xs)) τ) (Unfold %0)))) ,
+                     Lam (Fold (Snd (embed_project_pair (1 :: ((+2) <$> xs)) τ) (Unfold (extract TCRec %0)))))%Eₙₒ
+  | TVar X => match xs !! X with
+             | Some x => Var x
+             | None => dummy
+             end
+  | TForall τ => dummy
+  end.
+
+Lemma embed_project_pair_typed_gen (τ : type) (τs : list type) (pτn : Closed_n (length τs) τ) (xs : list var) Γ
+      (P : Forall2 (fun x τ => Γ !! x = Some ((τ ⟶ TUniverse) × (TUniverse ⟶ τ))%Tₙₒ) xs τs) :
+  Γ ⊢ₙₒ (embed_project_pair xs τ) : ((τ.[subst_list τs] ⟶ TUniverse) × (TUniverse ⟶ τ.[subst_list τs])).
+Proof.
+  generalize dependent Γ.
+  generalize dependent xs.
+  generalize dependent τs.
+  induction τ as [ | | | τ1 IHτ1 τ2 IHτ2 | τ1 IHτ1 τ2 IHτ2 | τ1 IHτ1 τ2 IHτ2 | τb IHτb | X | sadf ] ;
+    intros τs Cnτ xs Γ Pxsτs; try by repeat (apply Pair_typed || apply inject_typed || apply extract_typed).
+  - (* TProd *) assert (pCτ1 : Closed_n (length τs) τ1). admit. assert (pCτ2 : Closed_n (length τs) τ2). admit.
+    specialize (IHτ1 τs pCτ1). specialize (IHτ2 τs pCτ2).
+    apply Pair_typed; fold embed_project_pair;
+      repeat (apply IHτ1 || apply IHτ2 || apply inject_typed || apply extract_typed || econstructor); by apply Forall2_fmap_l.
+  - (* TSum *) assert (pCτ1 : Closed_n (length τs) τ1). admit. assert (pCτ2 : Closed_n (length τs) τ2). admit.
+    specialize (IHτ1 τs pCτ1). specialize (IHτ2 τs pCτ2).
+    apply Pair_typed; fold embed_project_pair;
+      repeat (apply IHτ1 || apply IHτ2 || apply inject_typed || apply (extract_typed TCSum) || econstructor); by apply Forall2_fmap_l.
+  - (* TArrow *) assert (pCτ1 : Closed_n (length τs) τ1). admit. assert (pCτ2 : Closed_n (length τs) τ2). admit.
+    specialize (IHτ1 τs pCτ1). specialize (IHτ2 τs pCτ2).
+    apply Pair_typed; fold embed_project_pair;
+      repeat (apply IHτ1 || apply IHτ2 || apply inject_typed || apply (extract_typed TCArrow) || econstructor); by apply Forall2_fmap_l.
+  - (* TRec *) specialize (IHτb ((TRec τb).[subst_list τs] :: τs)).
+    assert (Closed_n (S (length τs)) τb) as CSnτb. admit. specialize (IHτb CSnτb).
+    assert (τb.[up (subst_list τs)].[TRec τb.[up (subst_list τs)]/] = τb.[subst_list ((TRec τb).[subst_list τs] :: τs)]) as eqn.
+      { rewrite -subst_list_cons_closed_S_n_type. by asimpl. done. }
+    apply FixLam_typed. fold (embed_project_pair). apply Pair_typed.
+    + apply Lam_typed. apply App_typed with (τ1 := TRec TUniverse). apply inject_typed. apply Fold_typed.
+      apply App_typed with (τ1 := τb.[up (subst_list τs)].[TRec τb.[up (subst_list τs)]/]).
+      eapply Fst_typed. rewrite eqn. apply IHτb. simpl. apply Forall2_cons. split.
+      apply Forall2_fmap_l. apply (Forall2_impl _ _ _ _ Pxsτs). by simpl.
+      apply Unfold_typed. by apply Var_typed.
+    + apply Lam_typed. apply Fold_typed. apply App_typed with (τ1 := TUniverse). eapply Snd_typed.
+      rewrite eqn. apply IHτb. simpl. apply Forall2_cons. split.
+      apply Forall2_fmap_l. apply (Forall2_impl _ _ _ _ Pxsτs). by simpl.
+      assert (TUniverse = TUniverse.[TRec TUniverse/]) as ->. intros; by asimpl. apply Unfold_typed. eapply App_typed. apply extract_typed. by apply Var_typed.
+  - (* TVar *) assert (X < (length τs)) as pxltlτs. admit. simpl. destruct (xs !! X) as [x |] eqn:eq.
+    + apply Var_typed. rewrite /subst_list. destruct (τs !! X) as [τ |] eqn:eq2.
+      * simpl. apply (Forall2_lookup_lr _ _ _ X _ _ Pxsτs eq eq2).
+      * exfalso. assert (length xs = length τs). by eapply Forall2_length.
+        assert (length τs ≤ X). by eapply lookup_ge_None_1.
+        assert (X < length xs). by eapply lookup_lt_Some. lia.
+    + exfalso. assert (length xs = length τs). by eapply Forall2_length.
+        assert (length xs ≤ X). by eapply lookup_ge_None_1. lia.
+Admitted.
+
+Lemma embed_project_pair_typed (τ : type) (pτ : Closed τ) Γ :
+  Γ ⊢ₙₒ (embed_project_pair [] τ) : ((τ ⟶ TUniverse) × (TUniverse ⟶ τ)).
+Proof.
+  cut (Γ ⊢ₙₒ embed_project_pair [] τ : (τ.[subst_list []] ⟶ TUniverse) × (TUniverse ⟶ τ.[subst_list []])); first by rewrite pτ.
+  by apply embed_project_pair_typed_gen.
+Qed.
+
+(* (* If we somehow end up only allowing closed types... *) *)
+
+(* Lemma embed_project_pair_typed_closed_gen (τ : type) (τs : list type) (pτn : Closed_n (length τs) τ) (xs : list var) Γ *)
+(*       (P : Forall2 (fun x τ => Closed τ ∧ Γ !! x = Some ((τ ⟶ TUniverse) × (TUniverse ⟶ τ))%Tₙₒ) xs τs) : *)
+(*   Γ ⊢ₙₒ (embed_project_pair xs τ) : ((τ.[subst_list τs] ⟶ TUniverse) × (TUniverse ⟶ τ.[subst_list τs])). *)
+(* Proof. *)
+(*   generalize dependent Γ. *)
+(*   generalize dependent xs. *)
+(*   generalize dependent τs. *)
+(*   induction τ as [ | | | τ1 IHτ1 τ2 IHτ2 | τ1 IHτ1 τ2 IHτ2 | τ1 IHτ1 τ2 IHτ2 | τb IHτb | X | sadf ] ; *)
+(*     intros τs Cnτ xs Γ Pxsτs; try by repeat (apply Pair_typed || apply inject_typed || apply extract_typed). *)
+(*   - (* TProd *) assert (pCτ1 : Closed_n (length τs) τ1). admit. assert (pCτ2 : Closed_n (length τs) τ2). admit. *)
+(*     specialize (IHτ1 τs pCτ1). specialize (IHτ2 τs pCτ2). *)
+(*     apply Pair_typed; fold embed_project_pair; *)
+(*       repeat (apply IHτ1 || apply IHτ2 || apply inject_typed || apply extract_typed || econstructor); by apply Forall2_fmap_l. *)
+(*   - (* TSum *) assert (pCτ1 : Closed_n (length τs) τ1). admit. assert (pCτ2 : Closed_n (length τs) τ2). admit. *)
+(*     specialize (IHτ1 τs pCτ1). specialize (IHτ2 τs pCτ2). *)
+(*     apply Pair_typed; fold embed_project_pair; *)
+(*       repeat (apply IHτ1 || apply IHτ2 || apply inject_typed || apply (extract_typed TCSum) || econstructor); by apply Forall2_fmap_l. *)
+(*   - (* TArrow *) assert (pCτ1 : Closed_n (length τs) τ1). admit. assert (pCτ2 : Closed_n (length τs) τ2). admit. *)
+(*     specialize (IHτ1 τs pCτ1). specialize (IHτ2 τs pCτ2). *)
+(*     apply Pair_typed; fold embed_project_pair; *)
+(*       repeat (apply IHτ1 || apply IHτ2 || apply inject_typed || apply (extract_typed TCArrow) || econstructor); by apply Forall2_fmap_l. *)
+(*   - (* TRec *) specialize (IHτb ((TRec τb).[subst_list τs] :: τs)). *)
+(*     assert (Closed (TRec τb).[subst_list τs]) as pCμτb. admit. *)
+(*     assert (Closed_n (S (length τs)) τb) as CSnτb. admit. specialize (IHτb CSnτb). *)
+(*     assert (τb.[up (subst_list τs)].[TRec τb.[up (subst_list τs)]/] = τb.[subst_list ((TRec τb).[subst_list τs] :: τs)]) as eqn. *)
+(*       { rewrite -subst_list_cons_closed_S_n_type. by asimpl. done. } *)
+(*     apply FixLam_typed. fold (embed_project_pair). apply Pair_typed. *)
+(*     + apply Lam_typed. apply App_typed with (τ1 := TRec TUniverse). apply inject_typed. apply Fold_typed. *)
+(*       apply App_typed with (τ1 := τb.[up (subst_list τs)].[TRec τb.[up (subst_list τs)]/]). *)
+(*       eapply Fst_typed. rewrite eqn. apply IHτb. apply Forall2_cons. split; try by simpl. *)
+(*       apply Forall2_fmap_l. apply (Forall2_impl _ _ _ _ Pxsτs). by simpl. *)
+(*       apply Unfold_typed. by apply Var_typed. *)
+(*     + apply Lam_typed. apply Fold_typed. apply App_typed with (τ1 := TUniverse). eapply Snd_typed. *)
+(*       rewrite eqn. apply IHτb. simpl. apply Forall2_cons. split; try by simpl. *)
+(*       apply Forall2_fmap_l. apply (Forall2_impl _ _ _ _ Pxsτs). by simpl. *)
+(*       assert (TUniverse = TUniverse.[TRec TUniverse/]) as ->. intros; by asimpl. apply Unfold_typed. eapply App_typed. apply extract_typed. by apply Var_typed. *)
+(*   - (* TVar *) assert (X < (length τs)) as pxltlτs. admit. simpl. destruct (xs !! X) as [x |] eqn:eq. *)
+(*     + apply Var_typed. rewrite /subst_list. destruct (τs !! X) as [τ |] eqn:eq2. *)
+(*       * simpl. apply (Forall2_lookup_lr _ _ _ X _ _ Pxsτs eq eq2). *)
+(*       * exfalso. assert (length xs = length τs). by eapply Forall2_length. *)
+(*         assert (length τs ≤ X). by eapply lookup_ge_None_1. *)
+(*         assert (X < length xs). by eapply lookup_lt_Some. lia. *)
+(*     + exfalso. assert (length xs = length τs). by eapply Forall2_length. *)
+(*         assert (length xs ≤ X). by eapply lookup_ge_None_1. lia. *)
+(* Admitted. *)
