theories/lam/types.v
@@ -1,0 +1,37 @@
+From st Require Export autosubst.
+
+Inductive type :=
+ | TUnit : type
+ | TBool : type
+ | TInt : type
+ | TProd (τ1 τ2 : type) : type
+ | TSum (τ1 τ2 : type) : type
+ | TArrow (τ1 τ2 : type) : type
+ | TRec (τ : {bind 1 of type})
+ | TVar (X : var)
+ | TForall (τ : {bind 1 of type}).
+
+Global Instance type_eq_dec (τ τ' : type) : Decision (τ = τ').
+Proof. solve_decision. Defined.
+
+Instance Ids_type : Ids type. derive. Defined.
+Instance Rename_type : Rename type. derive. Defined.
+Instance Subst_type : Subst type. derive. Defined.
+Instance SubstLemmas_typer : SubstLemmas type. derive. Qed.
+
+Declare Scope types_nost_scope.
+
+Infix "×" := TProd (at level 49) : types_no_st_scope.
+Infix "+" := TSum : types_no_st_scope.
+Infix "⟶" := TArrow (at level 51) : types_no_st_scope.
+
+Delimit Scope types_no_st_scope with Tₙₒ.
+
+Lemma test : (TProd (TVar 0) (TVar 1)).[TBool, TInt/] = TProd TBool TInt.
+Proof. by simpl. Qed.
+
+Lemma test' : (TProd (TVar 0) (TVar 1)).[TBool/].[TInt/] = TProd TBool TInt.
+Proof. by simpl. Qed.
+
+(* Lemma test'' : (TVar 0).[TVar 0/].[TInt/] = (TVar 0).[TVar 0,TInt/]. *)
+(* Proof. simpl. Qed. *)
