theories/lamst/types.v
@@ -1,0 +1,30 @@
+From st Require Export autosubst.
+
+Inductive type :=
+ | TUnit : type
+ | TBool : type
+ | TInt : type
+ | TProd : type → type → type
+ | TSum : type → type → type
+ | TArrow : type → type → type
+ | TRec (τ : {bind 1 of type})
+ | TVar (X : var)
+ | TForall (τ : {bind 1 of type})
+ | TSTref (ρ τ : type)
+ | TST (ρ τ : type).
+
+Global Instance type_eq_dec (τ τ' : type) : Decision (τ = τ').
+Proof. solve_decision. Defined.
+
+Instance Ids_type : Ids type. derive. Defined.
+Instance Rename_type : Rename type. derive. Defined.
+Instance Subst_type : Subst type. derive. Defined.
+Instance SubstLemmas_typer : SubstLemmas type. derive. Qed.
+
+Declare Scope types_nost_scope.
+
+Infix "×" := TProd (at level 99) : types_st_scope.
+Infix "+" := TSum : types_st_scope.
+Infix "⟶" := TArrow (at level 100) : types_st_scope.
+
+Delimit Scope types_st_scope with Tₛₜ.
